jwnlgj

.lake/build/ir/Games/gameLib/Stealing.c
@@ -1,6 +1,6 @@
 // Lean compiler output
-// Module: Games.gameLib.Zermelo
-// Imports: Init Games.gameLib.ConwayInduction
+// Module: Games.gameLib.Stealing
+// Imports: Init Games.gameLib.Zermelo
 #include <lean/lean.h>
 #if defined(__clang__)
 #pragma clang diagnostic ignored "-Wunused-parameter"
@@ -14,16 +14,16 @@
 extern "C" {
 #endif
 lean_object* initialize_Init(uint8_t builtin, lean_object*);
-lean_object* initialize_Games_gameLib_ConwayInduction(uint8_t builtin, lean_object*);
+lean_object* initialize_Games_gameLib_Zermelo(uint8_t builtin, lean_object*);
 static bool _G_initialized = false;
-LEAN_EXPORT lean_object* initialize_Games_gameLib_Zermelo(uint8_t builtin, lean_object* w) {
+LEAN_EXPORT lean_object* initialize_Games_gameLib_Stealing(uint8_t builtin, lean_object* w) {
 lean_object * res;
 if (_G_initialized) return lean_io_result_mk_ok(lean_box(0));
 _G_initialized = true;
 res = initialize_Init(builtin, lean_io_mk_world());
 if (lean_io_result_is_error(res)) return res;
 lean_dec_ref(res);
-res = initialize_Games_gameLib_ConwayInduction(builtin, lean_io_mk_world());
+res = initialize_Games_gameLib_Zermelo(builtin, lean_io_mk_world());
 if (lean_io_result_is_error(res)) return res;
 lean_dec_ref(res);
 return lean_io_result_mk_ok(lean_box(0));
