Games/games/Chomp.lean
@@ -4,15 +4,27 @@ Released under Apache 2.0 license as described in the file LICENSE.
 Author: Yves Jäckle.
 -/
 
-import Games.exLib.List
-import Games.gameLib.Conditioning_Symm
-import Mathlib.Tactic
-import Mathlib.Data.List.ProdSigma
---import Games.gameLib.Stealing_Symm
-import Games.gameLib.Zermelo_Symm
+import Games.gameLib.Stealing
+
+#exit
+/-
+This file describes the game of Chomp and proves that the first player has a winning strategy for it.
+The game of chomp is played on a `hight` × `length` grid-like board. At each turn, a player may select
+a tile of the board. From there on, all tiles dominated (wrt. lexicographic order) by that tile may not
+be selected anymore (think of the board as of a chocolate bar, who's tiles are getting "chomped" off).
+The player that eats the last tile loses the game.
+
+The main concept are:
+- `preChomp` defines the game of chomp, `Chomp` glues the Zermelo properties to it
+- `Chomp_stealing_condition` shows that Chomp satisfies the stealing conditions
+- `Chomp_is_fst_win` show that Chomp has a winning strategy for the first player, via strategy stealing.
+
+-/
 
 
+-- # Chomp state lemmata
 
+/-- a grid-point is dominated by another if both its coordinates are smaller-/
 def domi (p q : ℕ × ℕ) : Prop := p.1 ≤ q.1 ∧ p.2 ≤ q.2
 
 def nondomi (p q : ℕ × ℕ) : Prop := ¬ domi p q
@@ -36,8 +48,9 @@ instance (l : List (ℕ × ℕ)) : DecidablePred (fun p => ∀ q ∈ l, nondomi 
   exact List.decidableBAll (fun x => ¬(x.1 ≤ p.1 ∧ x.2 ≤ p.2)) l
 
 
-
-
+/-- The current board is obtained by considering all tiles from the
+initial board, that aren't dominated by a tile played sofar
+-/
 def Chomp_state (ini : Finset (ℕ × ℕ)) (hist : List (ℕ × ℕ)) :=
   ini.filter (fun p => ∀ q ∈ hist, nondomi q p)
 
@@ -66,6 +79,7 @@ lemma Chomp_state_sub' (ini : Finset (ℕ × ℕ)) (l L :  List (ℕ × ℕ)) :
     apply xdef.2
     exact List.mem_append_right l ql
 
+
 lemma Chomp_state_sub_cons (ini : Finset (ℕ × ℕ)) (x : ℕ × ℕ) (l :  List (ℕ × ℕ)) :
   Chomp_state ini (x :: l) ⊆ Chomp_state ini l :=
   by
@@ -85,106 +99,24 @@ lemma Chomp_state_sub_of_hist_sub (ini : Finset (ℕ × ℕ)) (l L :  List (ℕ 
     apply xdef.2
     exact h ql
 
+-- to mathlib
+lemma List.mem_of_suffix  {a b : List α} {x : α} (ha : a <:+ b) (hx : x ∈ a) : x ∈ b := by
+  obtain ⟨t,tdef⟩ := ha ; rw [← tdef, List.mem_append] ; right ; exact hx
+
+-- to mathlib
+lemma List.subset_of_suffix  {a b : List α} (ha : a <:+ b) : a ⊆ b := by
+  intro x xa ; apply List.mem_of_suffix ha xa
 
 
+lemma Chomp_state_sub_of_hist_suffix (ini : Finset (ℕ × ℕ)) (l L :  List (ℕ × ℕ)) (h : l <:+ L) :
+  Chomp_state ini (L) ⊆ Chomp_state ini l :=
+  by apply Chomp_state_sub_of_hist_sub ; apply List.subset_of_suffix h
+
+
+/-- The initial board is a rectangle-/
 def Chomp_init (height length : ℕ) := (Finset.range (length+1)) ×ˢ (Finset.range (height+1))
 
-lemma Chomp_state_blind (ini : Finset (ℕ × ℕ)) (hist prehist : List (ℕ × ℕ)) :
-  Chomp_state (Chomp_state ini prehist) hist = Chomp_state ini (hist ++ prehist) :=
-  by
-  ext x
-  constructor
-  · intro H
-    dsimp [Chomp_state] at *
-    simp_rw [Finset.mem_filter] at *
-    constructor
-    · exact H.1.1
-    · intro q qq
-      rw [List.mem_append] at qq
-      cases' qq with k k
-      · exact H.2 q k
-      · exact H.1.2 q k
-  · intro H
-    dsimp [Chomp_state] at *
-    simp_rw [Finset.mem_filter] at *
-    constructor
-    · constructor
-      · exact H.1
-      · intro q qh
-        apply H.2
-        exact List.mem_append_right hist qh
-    · intro q qh
-      apply H.2
-      exact List.mem_append.mpr (Or.inl qh)
 
-
-
-
-
-structure Chomp_law (ini : Finset (ℕ × ℕ)) (hist : List (ℕ × ℕ)) (act : ℕ × ℕ) : Prop where
-  act_mem : act ∈ ini
-  hist_mem : ∀ q ∈ hist, q ∈ ini
-  hist_nd : List.Pairwise (fun x y => nondomi y x) hist
-  nd : ∀ q ∈ hist, nondomi q act
-  nz_act : act ≠ (0,0)
-
-
-def preChomp (height length : ℕ) : Symm_Game_World (Finset (ℕ × ℕ)) (ℕ × ℕ) where
-  init_game_state := Chomp_init height length
-  win_states := (fun state => state = {(0,0)})
-  transition := fun ini hist act => if Chomp_state ini hist ≠ {(0,0)}
-                                    then (Chomp_state ini) (act :: hist)
-                                    else {(0,0)}
-  law := fun ini hist act => if (0,0) ∈ ini ∧ (0,0) ∉ hist
-                             then
-                              if Chomp_state ini hist ≠ {(0,0)}
-                              then Chomp_law ini hist act
-                              else act ≠ (0,0) -- saves ass in `preChomp_law_careless`
-                             else True
-
---#exit
-
-lemma Chomp_state_ini_zero (hist : List (ℕ × ℕ)) (hh : (0,0) ∉ hist): Chomp_state {(0,0)} hist = {(0,0)} :=
-  by
-  dsimp [Chomp_state]
-  rw [Finset.filter_eq_self]
-  intro x xdef q qh
-  rw [Finset.mem_singleton] at xdef
-  rw [xdef]
-  dsimp [nondomi, domi]
-  intro con
-  simp_rw [Nat.le_zero] at con
-  apply hh
-  convert qh
-  · exact con.1.symm
-  · exact con.2.symm
-
-lemma Chomp_state_has_zero_iff_hist_has_zero
-  (ini : Finset (ℕ × ℕ) ) (hini : (0,0) ∈ ini) (hist : List (ℕ × ℕ)) :
-  (0,0) ∈ Chomp_state ini hist ↔ (0,0) ∉ hist :=
-  by
-  constructor
-  · intro c
-    dsimp [Chomp_state] at c
-    rw [Finset.mem_filter] at c
-    dsimp [nondomi, domi] at c
-    intro con
-    apply c.2 _ con
-    decide
-  · intro c
-    dsimp [Chomp_state]
-    rw [Finset.mem_filter]
-    constructor
-    · exact hini
-    · intro q qh
-      dsimp [nondomi, domi]
-      intro con
-      simp_all only [nonpos_iff_eq_zero]
-      unhygienic with_reducible aesop_destruct_products
-      simp_all only
-
-lemma Chomp_state_sub_ini (ini : Finset (ℕ × ℕ) ) (hist : List (ℕ × ℕ)) :
-  Chomp_state ini hist ⊆ ini := by dsimp [Chomp_state]; exact Finset.filter_subset (fun p => ∀ q ∈ hist, nondomi q p) ini
 
 lemma Chomp_state_hist_zero (ini : Finset (ℕ × ℕ) ) (hist : List (ℕ × ℕ)) (main : (0,0) ∈ hist) :
   Chomp_state ini hist = ∅ :=
@@ -210,55 +142,6 @@ lemma Chomp_state_state_empty (ini : Finset (ℕ × ℕ) ) (hini : (0,0) ∈ ini
   simp only [nonpos_iff_eq_zero] at *
   convert qh <;> {rw [eq_comm] ; assumption}
 
-
-
-lemma Chomp_law_state_mem (ini : Finset (ℕ × ℕ) ) (hist : List (ℕ × ℕ)) (act : ℕ × ℕ) (leg : Chomp_law ini hist act) :
-  act ∈ Chomp_state ini hist :=
-  by
-  dsimp [Chomp_state]
-  rw [Finset.mem_filter]
-  constructor
-  · exact leg.act_mem
-  · exact leg.nd
-
-
-lemma Chomp_law_sub (ini : Finset (ℕ × ℕ) ) (l L : List (ℕ × ℕ)) (act : ℕ × ℕ) (leg : Chomp_law ini (l ++ L) act) :
-  Chomp_law ini L act :=
-  by
-  refine' ⟨leg.act_mem, _, _,  _ , leg.nz_act⟩
-  · intro q qdef
-    apply leg.hist_mem
-    exact List.mem_append_right l qdef
-  · have := leg.hist_nd
-    rw [List.pairwise_append] at this
-    exact this.2.1
-  · intro q qdef
-    apply leg.nd
-    exact List.mem_append_right l qdef
-
-
-
-
-lemma Chomp_hist_no_zero_of_Hist_legal (height length : ℕ) (ini : Finset (ℕ × ℕ) ) (hini : (0,0) ∈ ini) (prehist : List (ℕ × ℕ))
-  (main : Hist_legal (preChomp height length).law (preChomp height length).law ini prehist) : (0,0) ∉ prehist :=
-  by
-  induction' prehist with x l ih
-  · decide
-  · cases' main
-    rename_i sofar now
-    apply List.not_mem_cons_of_ne_of_not_mem
-    · split_ifs at now
-      all_goals { dsimp [preChomp] at now
-                  rw [if_pos ⟨hini, ih sofar⟩ ] at now
-                  split_ifs at now
-                  · contrapose! now
-                    apply now.symm
-                  · rw [ne_comm]
-                    apply now.nz_act}
-    · exact ih sofar
-
-
-
 lemma nondomi_zero (act : ℕ × ℕ) : nondomi act (0,0) ↔ act ≠ (0,0) := by
   dsimp [nondomi,domi]
   simp_rw [Nat.le_zero]
@@ -268,748 +151,12 @@ lemma nondomi_zero (act : ℕ × ℕ) : nondomi act (0,0) ↔ act ≠ (0,0) := b
 
 
 
-lemma Chomp_state_zero_act_non_zero (ini : Finset (ℕ × ℕ)) (hini : (0, 0) ∈ ini) (hist : List (ℕ × ℕ)) (act : ℕ × ℕ)
-  (hs : Chomp_state ini hist = {(0,0)}) (ha : act ≠ (0,0)) : Chomp_state ini (act :: hist) = {(0,0)} :=
-  by
-  dsimp [Chomp_state] at *
-  have : (fun p => ∀ q ∈ act :: hist, nondomi q p) = (fun p => (nondomi act p) ∧ (∀ q ∈ hist, nondomi q p)) :=
-    by
-    ext p
-    simp_all only [Prod.forall, List.mem_cons, forall_eq_or_imp]
-    unhygienic with_reducible aesop_destruct_products
-    simp_all only [Prod.forall, Prod.mk.injEq, not_and]
-    apply Iff.intro
-    · intro a
-      simp_all only [Prod.forall, and_self, true_or, or_true, implies_true, forall_const]
-    · intro a a_1 b a_2
-      unhygienic with_reducible aesop_destruct_products
-      unhygienic aesop_cases a_2
-      · simp_all only [Prod.forall]
-      · simp_all only [Prod.forall]
-  simp_rw [this, Finset.filter_and,hs]
-  rw [Finset.inter_eq_right]
-  intro y ydef
-  rw [Finset.mem_singleton] at ydef
-  rw [ydef, Finset.mem_filter]
-  exact ⟨ hini, (by rw [nondomi_zero]; exact ha)⟩
-
-lemma Chomp_hist_mem_ini_of_Hist_legal (height length : ℕ) (ini : Finset (ℕ × ℕ) ) (hini : (0,0) ∈ ini) (prehist : List (ℕ × ℕ))
-  (main : Hist_legal (preChomp height length).law (preChomp height length).law ini prehist)
-  (main' : Chomp_state ini prehist.tail ≠ {(0,0)}): ∀ q ∈ prehist, q ∈ ini :=
-  by
-  cases' prehist with x l
-  · intro q no ; contradiction
-  · intro q qdef
-    rw [List.tail_cons] at main'
-    cases' main
-    rename_i sofar now
-    rw [ite_self] at now
-    rw [List.mem_cons] at qdef
-    cases' qdef with qdef qdef
-    · rw [qdef]
-      dsimp [preChomp] at now
-      rw [if_pos ⟨hini, Chomp_hist_no_zero_of_Hist_legal height length ini hini l sofar⟩ ] at now
-      rw [if_pos main'] at now
-      exact now.act_mem
-    · dsimp [preChomp] at now
-      rw [if_pos ⟨hini, Chomp_hist_no_zero_of_Hist_legal height length ini hini l sofar⟩ ] at now
-      rw [if_pos main'] at now
-      exact now.hist_mem _ qdef
-
-
-
---#exit
-
-lemma Chomp_law_blind (ini : Finset (ℕ × ℕ) ) (l L : List (ℕ × ℕ)) (act : ℕ × ℕ) (c : Chomp_law ini (l ++ L) act) :
-  Chomp_law (Chomp_state ini L) l act :=
-  by
-  constructor
-  · dsimp [Chomp_state]
-    rw [Finset.mem_filter]
-    constructor
-    · exact c.act_mem
-    · intro e eh
-      apply c.nd
-      exact List.mem_append_right l eh
-  · intro q qdef
-    dsimp [Chomp_state]
-    rw [Finset.mem_filter]
-    constructor
-    · exact c.hist_mem q (by exact List.mem_append.mpr (Or.inl qdef))
-    · intro e eh
-      have := c.hist_nd
-      rw [List.pairwise_append] at this
-      apply this.2.2
-      · exact qdef
-      · exact eh
-  · have := c.hist_nd
-    rw [List.pairwise_append] at this
-    exact this.1
-  · intro e eh
-    apply c.nd
-    exact List.mem_append_left L eh
-  · apply c.nz_act
-
-
-
-lemma Chomp_hist_pairwise_nondomi_of_Hist_legal (height length : ℕ) (ini : Finset (ℕ × ℕ) ) (hini : (0,0) ∈ ini) (prehist : List (ℕ × ℕ))
-  (main : Hist_legal (preChomp height length).law (preChomp height length).law ini prehist)
-  (main' : Chomp_state ini prehist.tail ≠ {(0,0)}) : List.Pairwise (fun x y => nondomi y x) prehist :=
-  by
-  cases' prehist with x l
-  · apply List.Pairwise.nil
-  · cases' main
-    rename_i sofar now
-    rw [ite_self] at now
-    dsimp [preChomp] at now
-    rw [if_pos ⟨hini, Chomp_hist_no_zero_of_Hist_legal height length ini hini l sofar⟩ ] at now
-    rw [List.tail_cons] at main'
-    rw [ if_pos main'] at now
-    apply List.Pairwise.cons
-    · exact now.nd
-    · exact now.hist_nd
-
-
---#exit
-
-lemma Chomp_law_blind' (height length : Nat) (ini : Finset (ℕ × ℕ) ) (hini : (0,0) ∈ ini) (l L : List (ℕ × ℕ)) (act : ℕ × ℕ)
-  (leg : Hist_legal (preChomp height length).law (preChomp height length).law ini L) (c : Chomp_law (Chomp_state ini L) l act) :
-  Chomp_law ini (l ++ L) act  :=
-  by
-  constructor
-  · apply Chomp_state_sub_ini _ _ c.act_mem
-  · intro q qdef
-    have := c.hist_mem
-    specialize this q
-    dsimp [Chomp_state] at this
-    rw [Finset.mem_filter] at this
-    rw [List.mem_append] at qdef
-    cases' qdef with qdef qdef
-    · exact (this qdef).1
-    · cases' L with x L
-      · contradiction
-      · have that : Chomp_state ini (x :: L).tail ≠ {(0,0)} :=
-          by
-          intro con
-          cases' leg
-          rename_i sofar now
-          rw [ite_self] at now
-          dsimp [preChomp] at now
-          rw [if_pos ⟨hini, Chomp_hist_no_zero_of_Hist_legal height length ini hini L sofar⟩] at now
-          rw [if_neg (by rw [not_not] ; apply con)] at now
-          have fact := Chomp_state_zero_act_non_zero ini hini L x con now
-          rw [fact] at c
-          apply c.nz_act
-          replace c := c.act_mem
-          rw [Finset.mem_singleton] at c
-          exact c
-        exact Chomp_hist_mem_ini_of_Hist_legal height length ini hini (x :: L) leg that q qdef
-  · rw [List.pairwise_append]
-    constructor
-    · apply c.hist_nd
-    · constructor
-      · cases' L with x L
-        · apply List.Pairwise.nil
-        · have that : Chomp_state ini (x :: L).tail ≠ {(0,0)} :=
-            by
-            intro con
-            cases' leg
-            rename_i sofar now
-            rw [ite_self] at now
-            dsimp [preChomp] at now
-            rw [if_pos ⟨hini, Chomp_hist_no_zero_of_Hist_legal height length ini hini L sofar⟩] at now
-            rw [if_neg (by rw [not_not] ; apply con)] at now
-            have fact := Chomp_state_zero_act_non_zero ini hini L x con now
-            rw [fact] at c
-            apply c.nz_act
-            replace c := c.act_mem
-            rw [Finset.mem_singleton] at c
-            exact c
-          exact Chomp_hist_pairwise_nondomi_of_Hist_legal height length ini hini (x :: L) leg that
-      · intro a al b bL
-        replace c := c.hist_mem a al
-        dsimp [Chomp_state] at c
-        rw [Finset.mem_filter] at c
-        exact c.2 b bL
-  · intro q qdef
-    rw [List.mem_append] at qdef
-    cases' qdef with qdef qdef
-    · apply c.nd q qdef
-    · replace c := c.act_mem
-      dsimp [Chomp_state] at c
-      rw [Finset.mem_filter] at c
-      exact c.2 q qdef
-  · exact c.nz_act
-
-
-
-lemma preChomp_law_careless (height length : ℕ) :
-  careless (preChomp height length).law (preChomp height length).law (preChomp height length).init_game_state (preChomp height length).law (preChomp height length).transition :=
-  by
-  intro ini hist prehist pHne pHl
-  ext act
-  by_cases fix : (0,0) ∈ ini ∧ (0, 0) ∉ hist
-  · constructor
-    · intro c
-      dsimp [preChomp] at c
-      rw [if_pos ⟨fix.1, (by apply List.not_mem_append fix.2 ; exact Chomp_hist_no_zero_of_Hist_legal height length ini fix.1 prehist pHl)⟩ ] at c
-      by_cases q1 : Chomp_state ini (hist ++ prehist) ≠ {(0,0)}
-      · rw [if_pos q1] at c
-        by_cases q2 : Chomp_state (Symm_Game_World.transition (preChomp height length) ini (List.tail prehist) (List.head prehist pHne)) (hist) ≠ {(0,0)}
-        · dsimp [preChomp] at *
-          rw [if_pos q2]
-          rw [List.cons_head_tail] at *
-          by_cases q3 : Chomp_state ini (List.tail prehist) ≠ {(0, 0)}
-          · rw [if_pos q3] at *
-            split_ifs
-            all_goals { apply Chomp_law_blind _ _ _ _ c
-            }
-          · rw [if_neg q3] at *
-            exfalso
-            have : Chomp_state {(0, 0)} hist ⊂ {(0, 0)} :=
-              by
-              rw [Finset.ssubset_iff_subset_ne]
-              constructor
-              · apply Chomp_state_sub_ini
-              · exact q2
-            rw [Finset.ssubset_singleton_iff] at this
-            have that := Chomp_state_has_zero_iff_hist_has_zero {(0,0)} (by apply Finset.mem_singleton_self) hist
-            rw [iff_not_comm] at that
-            rw [this] at that
-            simp only [Finset.not_mem_empty, not_false_eq_true, iff_true] at that
-            have thut := c.nd (0,0) (by exact List.mem_append_left prehist that)
-            dsimp [nondomi, domi] at thut
-            apply thut
-            simp only [zero_le, and_self]
-        · dsimp [preChomp] at *
-          rw [if_neg q2]
-          split_ifs
-          all_goals apply c.nz_act
-      · rw [if_neg q1] at c
-        by_cases q2 : Chomp_state (Symm_Game_World.transition (preChomp height length) ini (List.tail prehist) (List.head prehist pHne)) (hist) ≠ {(0,0)}
-        · dsimp [preChomp] at *
-          rw [if_pos q2]
-          rw [not_not] at q1
-          rw [List.cons_head_tail] at *
-          by_cases q3 : Chomp_state ini (List.tail prehist) ≠ {(0, 0)}
-          · rw [if_pos q3] at *
-            exfalso
-            rw [Chomp_state_blind] at q2
-            exact q2 q1
-          · rw [if_neg q3] at *
-            exfalso
-            have : Chomp_state {(0, 0)} hist ⊂ {(0, 0)} :=
-              by
-              rw [Finset.ssubset_iff_subset_ne]
-              constructor
-              · apply Chomp_state_sub_ini
-              · exact q2
-            rw [Finset.ssubset_singleton_iff] at this
-            have that := Chomp_state_has_zero_iff_hist_has_zero {(0,0)} (by apply Finset.mem_singleton_self) hist
-            rw [iff_not_comm] at that
-            rw [this] at that
-            simp only [Finset.not_mem_empty, not_false_eq_true, iff_true] at that
-            have thut : (0,0) ∈ ini :=
-              by
-              have := Chomp_state_sub_ini ini (hist ++ prehist)
-              rw [q1] at this
-              apply this (Finset.mem_singleton_self (0,0))
-            have thus := Chomp_state_has_zero_iff_hist_has_zero ini thut (hist ++ prehist)
-            rw [q1] at thus
-            simp only [Finset.mem_singleton, List.mem_append, true_iff] at thus
-            apply thus
-            left
-            exact that
-        · dsimp [preChomp] at *
-          rw [if_neg q2]
-          split_ifs
-          all_goals apply c
-    · intro c
-      dsimp [preChomp] at *
-      rw [if_pos ⟨fix.1, (by apply List.not_mem_append fix.2 ; exact Chomp_hist_no_zero_of_Hist_legal height length ini fix.1 prehist pHl)⟩ ]
-      rw [List.cons_head_tail] at *
-      by_cases q1 : Chomp_state ini (hist ++ prehist) ≠ {(0,0)}
-      · rw [if_pos q1]
-        by_cases q2 : Chomp_state ini (List.tail prehist) ≠ {(0, 0)}
-        · rw [if_pos q2] at c
-          by_cases q3 : Chomp_state (Chomp_state ini prehist) hist ≠ {(0, 0)}
-          · rw [if_pos q3] at c
-            rw [if_pos ⟨(Chomp_state_has_zero_iff_hist_has_zero ini fix.1 prehist).mpr (Chomp_hist_no_zero_of_Hist_legal height length ini fix.1 prehist pHl) , fix.2⟩ ] at c
-            exact Chomp_law_blind' height length _ fix.1 _ _ _ pHl c
-          · rw [if_neg q3] at c
-            rw [not_not] at q3
-            exfalso
-            rw [Chomp_state_blind] at q3
-            exact q1 q3
-        · rw [if_neg q2] at c
-          by_cases q3 : Chomp_state {(0, 0)} hist ≠ {(0, 0)}
-          · rw [if_pos q3, if_pos ⟨ (by apply Finset.mem_singleton_self) , fix.2⟩ ] at c
-            exfalso
-            apply c.nz_act
-            have := c.act_mem
-            rwa [Finset.mem_singleton] at this
-          · rw [if_neg q3] at c
-            rw [not_not] at q3 q2
-            exfalso
-            have : (0,0) ∉ hist :=
-              by
-              intro con
-              have := Chomp_state_hist_zero {(0,0)} hist con
-              rw [this] at q3
-              contradiction
-            have temp : hist ++ prehist = (hist ++ [prehist.head pHne]) ++ prehist.tail :=
-              by rw [List.append_assoc, List.singleton_append, List.cons_head_tail]
-            rw [temp] at q1
-            have that := Chomp_state_sub' ini (hist ++ [prehist.head pHne]) prehist.tail
-            rw [q2] at that
-            rw [Finset.subset_singleton_iff] at that
-            cases' that with k k
-            · have fact : (0,0) ∈ ini :=
-                by
-                apply Chomp_state_sub_ini _ prehist.tail
-                rw [q2]
-                exact Finset.mem_singleton.mpr rfl
-              have more := Chomp_state_state_empty _ fact _ k
-              have thut : (0,0) ∉ prehist.tail :=
-                by
-                intro con
-                have tmp := Chomp_state_hist_zero ini _ con
-                rw [tmp] at q2
-                contradiction
-              rw [List.mem_append] at more
-              cases' more with more more
-              · rw [List.mem_append] at more
-                cases' more with more more
-                · exact this more
-                · rw [List.mem_singleton] at more
-                  cases' prehist with x l
-                  · contradiction
-                  · cases' pHl
-                    · rename_i uno dos
-                      by_cases last : Turn_fst (List.length l + 1)
-                      · rw [if_pos last, if_pos ⟨fix.1 , thut⟩ , if_neg (by rw [not_not] ; apply q2)] at dos
-                        apply dos
-                        rw [more]
-                        rfl
-                      · rw [if_neg last, if_pos  ⟨fix.1 , thut⟩, if_neg (by rw [not_not] ; apply q2)] at dos
-                        apply dos
-                        rw [more]
-                        rfl
-              · exact thut more
-            · exact q1 k
-      · rw [if_neg q1]
-        split_ifs at c
-        · exact c
-        · apply c.nz_act
-        · rename_i no
-          push_neg at no
-          exact False.elim (fix.2 (no (by apply Finset.mem_singleton_self)))
-        · exact c
-        · apply c.nz_act
-        · exfalso
-          rename_i no
-          apply no
-          rw [Chomp_state_has_zero_iff_hist_has_zero ini fix.1 prehist]
-          exact ⟨Chomp_hist_no_zero_of_Hist_legal height length ini fix.1 prehist pHl, fix.2⟩
-  · dsimp [preChomp]
-    rw [if_neg (by push_neg at * ;intro _ ; simp_all only [ne_eq, forall_true_left, List.mem_append, true_or] )]
-    simp only [ite_not, true_iff]
-    split_ifs
-    · rename_i a b c
-      rw [← a] at b
-      exact False.elim (by apply fix ; constructor ; apply Chomp_state_sub_ini ; apply b.1 ; apply b.2)
-    · rename_i a b c
-      rw [← a] at b
-      exact False.elim (by apply fix ; constructor ; apply Chomp_state_sub_ini ; apply b.1 ; apply b.2)
-    · rename_i a b c
-      exact False.elim (by apply fix ; constructor ; apply Chomp_state_sub_ini ; apply b.1 ; apply b.2)
-    · rename_i a b c
-      exact False.elim (by apply fix ; constructor ; apply Chomp_state_sub_ini ; apply b.1 ; apply b.2)
-
-
---#exit
-
-
-lemma preChomp_tranistion_careless (height length : ℕ) :
-  careless (preChomp height length).law (preChomp height length).law (preChomp height length).init_game_state (preChomp height length).transition (preChomp height length).transition :=
-  by
-  intro ini hist prehist pHne pHl
-  funext act
-  dsimp [preChomp]
-  by_cases q1 : Chomp_state ini (hist ++ prehist) ≠ {(0,0)}
-  · rw [if_pos q1] at *
-    by_cases q2 : Chomp_state ini (List.tail prehist) ≠ {(0, 0)}
-    · simp_rw [if_pos q2, List.cons_head_tail, Chomp_state_blind] at *
-      rw [if_pos q1, List.cons_append]
-    · simp_rw [if_neg q2] at *
-      by_cases q3 : Chomp_state {(0, 0)} hist ≠ {(0, 0)}
-      · rw [if_pos q3]
-        have : Chomp_state {(0, 0)} hist ⊂ {(0, 0)} :=
-            by
-            rw [Finset.ssubset_iff_subset_ne]
-            constructor
-            · apply Chomp_state_sub_ini
-            · exact q3
-        rw [Finset.ssubset_singleton_iff] at this
-        have that := Chomp_state_has_zero_iff_hist_has_zero {(0,0)} (by apply Finset.mem_singleton_self) hist
-        rw [iff_not_comm] at that
-        rw [this] at that
-        simp only [Finset.not_mem_empty, not_false_eq_true, iff_true] at that
-        have thut_l : (0,0) ∈ act :: (hist ++ prehist) :=
-          by apply List.mem_cons_of_mem ; apply List.mem_append_left ; exact that
-        rw [Chomp_state_hist_zero _ _ thut_l]
-        have thut_r : (0,0) ∈ act :: (hist) :=
-          by apply List.mem_cons_of_mem ; exact that
-        rw [Chomp_state_hist_zero _ _ thut_r]
-      · rw [if_neg q3, not_not] at *
-        exfalso
-        have : (0,0) ∉ hist :=
-            by
-            intro con
-            have := Chomp_state_hist_zero {(0,0)} hist con
-            rw [this] at q3
-            contradiction
-        have temp : hist ++ prehist = (hist ++ [prehist.head pHne]) ++ prehist.tail :=
-          by rw [List.append_assoc, List.singleton_append, List.cons_head_tail]
-        rw [temp] at q1
-        have that := Chomp_state_sub' ini (hist ++ [prehist.head pHne]) prehist.tail
-        rw [q2] at that
-        rw [Finset.subset_singleton_iff] at that
-        cases' that with k k
-        · have fact : (0,0) ∈ ini :=
-            by
-            apply Chomp_state_sub_ini _ prehist.tail
-            rw [q2]
-            exact Finset.mem_singleton.mpr rfl
-          have more := Chomp_state_state_empty _ fact _ k
-          have thut : (0,0) ∉ prehist.tail :=
-            by
-            intro con
-            have tmp := Chomp_state_hist_zero ini _ con
-            rw [tmp] at q2
-            contradiction
-          simp_rw [List.mem_append] at more
-          cases' more with more more
-          · cases' more with more more
-            · exact this more
-            · rw [List.mem_singleton] at more
-              cases' prehist with x l
-              · contradiction
-              · dsimp at *
-                cases' pHl
-                rename_i main
-                split_ifs at main
-                all_goals {dsimp [preChomp] at main ; rw [if_pos ⟨fact, thut⟩, if_neg (by rw [not_not] ; exact q2)] at main ; exact main more.symm}
-          · exact thut more
-        · exact q1 k
-  · rw [if_neg q1] at *
-    by_cases q2 : Chomp_state ini (List.tail prehist) ≠ {(0, 0)}
-    · simp_rw [if_pos q2, List.cons_head_tail, Chomp_state_blind] at *
-      rw [if_neg q1]
-    · simp_rw [if_neg q2] at *
-      by_cases q3 : Chomp_state {(0, 0)} hist ≠ {(0, 0)}
-      · exfalso
-        rw [not_not] at *
-        apply q3
-        apply Chomp_state_ini_zero hist
-        intro con
-        have := Chomp_state_hist_zero ini _ con
-        have that := Chomp_state_sub ini hist prehist
-        simp_all only [ne_eq, Finset.singleton_subset_iff, Finset.not_mem_empty]
-      · rw [not_not] at *
-        rw [if_neg (by rw [not_not] ; exact q3)]
-
-
-
 
 lemma Chomp_init_has_zero (height length : ℕ)  : (0,0) ∈ Chomp_init height length :=
   by
   dsimp [Chomp_init]
   simp_rw [Finset.mem_product, Finset.mem_range, and_comm]
   constructor <;> {exact Nat.add_pos_right _ Nat.le.refl}
-
-
-
-
-lemma preChomp_coherent (height length : ℕ)  : (preChomp height length).coherent_end :=
-  by
-  intro f_strat s_strat f_leg s_leg t main
-  dsimp [preChomp] at *
-  by_cases q1 : Turn_fst (t + 1)
-  · rw [Symm_Game_World.state_on_turn_fst_to_snd _ _ _ _ q1]
-    dsimp [preChomp]
-    rw [if_neg]
-    rw [not_not]
-    cases' t with t
-    · dsimp [Symm_Game_World.state_on_turn, Symm_Game_World.history_on_turn, History_on_turn] at *
-      simp_all only [zero_add]
-      rfl
-    · dsimp [Symm_Game_World.state_on_turn, Symm_Game_World.history_on_turn, History_on_turn] at main
-      rw [if_neg (by contrapose q1 ; rw [not_not] at q1 ; rw [← Turn_fst_not_step] ; exact q1)] at main
-      split_ifs at main with k
-      · dsimp [History_on_turn]
-        split_ifs with tu
-        · have : f_strat (Chomp_init height length) (History_on_turn (Chomp_init height length) f_strat s_strat t) ≠ (0, 0) :=
-            by
-            specialize f_leg t tu
-            by_cases split_ifs_is_wierd : ¬Chomp_state (Chomp_init height length) (History_on_turn (Chomp_init height length) f_strat s_strat t) = {(0, 0)}
-            · rw [if_pos ⟨(Chomp_init_has_zero _ _), (by rw [← Chomp_state_has_zero_iff_hist_has_zero (Chomp_init height length) (Chomp_init_has_zero _ _ ), k] ; apply Finset.mem_singleton_self )⟩ , if_pos (split_ifs_is_wierd)] at f_leg
-              exact f_leg.nz_act
-            · rw [if_pos ⟨(Chomp_init_has_zero _ _ ), (by rw [← Chomp_state_has_zero_iff_hist_has_zero (Chomp_init height length) (Chomp_init_has_zero _ _ ), k] ; apply Finset.mem_singleton_self )⟩, if_neg (split_ifs_is_wierd)] at f_leg
-              exact f_leg
-          apply Chomp_state_zero_act_non_zero
-          · exact Chomp_init_has_zero _ _
-          · exact k
-          · exact this
-        · have : s_strat (Chomp_init height length) (History_on_turn (Chomp_init height length) f_strat s_strat t) ≠ (0, 0) :=
-            by
-            specialize s_leg t tu
-            by_cases split_ifs_is_wierd : ¬Chomp_state (Chomp_init height length) (History_on_turn (Chomp_init height length) f_strat s_strat t) = {(0, 0)}
-            · rw [if_pos ⟨(Chomp_init_has_zero _ _ ), (by rw [← Chomp_state_has_zero_iff_hist_has_zero (Chomp_init height length) (Chomp_init_has_zero _ _ ), k] ; apply Finset.mem_singleton_self )⟩, if_pos (split_ifs_is_wierd)] at s_leg
-              exact s_leg.nz_act
-            · rw [if_pos ⟨(Chomp_init_has_zero _ _ ), (by rw [← Chomp_state_has_zero_iff_hist_has_zero (Chomp_init height length) (Chomp_init_has_zero _ _ ), k] ; apply Finset.mem_singleton_self )⟩, if_neg (split_ifs_is_wierd)] at s_leg
-              exact s_leg
-          apply Chomp_state_zero_act_non_zero
-          · exact Chomp_init_has_zero _ _
-          · exact k
-          · exact this
-      · dsimp [History_on_turn]
-        rw [if_neg (by rw [Turn_fst_not_step, not_not] ; exact q1)]
-        exact main
-  · rw [Turn_not_fst_iff_snd] at q1
-    rw [Symm_Game_World.state_on_turn_snd_to_fst _ _ _ _ q1]
-    dsimp [preChomp]
-    rw [if_neg]
-    rw [not_not]
-    cases' t with t
-    · dsimp [Symm_Game_World.state_on_turn, Symm_Game_World.history_on_turn, History_on_turn] at *
-      simp_all only [zero_add]
-      rfl
-    · dsimp [Symm_Game_World.state_on_turn, Symm_Game_World.history_on_turn, History_on_turn] at main
-      rw [if_pos (by contrapose q1 ; rw [← Turn_snd_not_step, ← Turn_not_fst_iff_snd] ; exact q1)] at main
-      split_ifs at main with k
-      · dsimp [History_on_turn]
-        split_ifs with tu
-        · have : f_strat (Chomp_init height length) (History_on_turn (Chomp_init height length) f_strat s_strat t) ≠ (0, 0) :=
-            by
-            specialize f_leg t tu
-            by_cases split_ifs_is_wierd : ¬Chomp_state (Chomp_init height length) (History_on_turn (Chomp_init height length) f_strat s_strat t) = {(0, 0)}
-            · rw [if_pos ⟨(Chomp_init_has_zero _ _ ), (by rw [← Chomp_state_has_zero_iff_hist_has_zero (Chomp_init height length) (Chomp_init_has_zero _ _ ), k] ; apply Finset.mem_singleton_self )⟩, if_pos (split_ifs_is_wierd)] at f_leg
-              exact f_leg.nz_act
-            · rw [if_pos ⟨(Chomp_init_has_zero _ _ ), (by rw [← Chomp_state_has_zero_iff_hist_has_zero (Chomp_init height length) (Chomp_init_has_zero _ _ ), k] ; apply Finset.mem_singleton_self )⟩, if_neg (split_ifs_is_wierd)] at f_leg
-              exact f_leg
-          apply Chomp_state_zero_act_non_zero
-          · exact Chomp_init_has_zero _ _
-          · exact k
-          · exact this
-        · have : s_strat (Chomp_init height length) (History_on_turn (Chomp_init height length) f_strat s_strat t) ≠ (0, 0) :=
-            by
-            specialize s_leg t tu
-            by_cases split_ifs_is_wierd : ¬Chomp_state (Chomp_init height length) (History_on_turn (Chomp_init height length) f_strat s_strat t) = {(0, 0)}
-            · rw [if_pos ⟨(Chomp_init_has_zero _ _ ), (by rw [← Chomp_state_has_zero_iff_hist_has_zero (Chomp_init height length) (Chomp_init_has_zero _ _ ), k] ; apply Finset.mem_singleton_self )⟩, if_pos (split_ifs_is_wierd)] at s_leg
-              exact s_leg.nz_act
-            · rw [if_pos ⟨(Chomp_init_has_zero _ _ ), (by rw [← Chomp_state_has_zero_iff_hist_has_zero (Chomp_init height length) (Chomp_init_has_zero _ _ ), k] ; apply Finset.mem_singleton_self )⟩, if_neg (split_ifs_is_wierd)] at s_leg
-              exact s_leg
-          apply Chomp_state_zero_act_non_zero
-          · exact Chomp_init_has_zero _ _
-          · exact k
-          · exact this
-      · dsimp [History_on_turn]
-        rw [if_pos (by rw [Turn_fst_not_step] ; exact q1)]
-        exact main
-
-
-lemma preChomp_playable (height length : ℕ) : (preChomp height length).playable :=
-  by
-  intro ini hist hist_leg
-  dsimp [preChomp]
-  by_cases q : ¬Chomp_state ini hist = {(0, 0)}
-  · simp_rw [if_pos q]
-    split_ifs
-    · have : ∃ act, act ∈ Chomp_state ini hist ∧ act ≠ (0,0) :=
-        by
-        contrapose! q
-        ext x
-        constructor
-        · intro xdef
-          specialize q x xdef
-          rename_i h
-          aesop_subst q
-          simp_all only [gt_iff_lt, Finset.mem_singleton]
-        · intro xdef
-          rw [Finset.mem_singleton] at xdef
-          rw [xdef]
-          dsimp [Chomp_state]
-          rw [Finset.mem_filter]
-          rename_i gain
-          refine' ⟨gain.1, _ ⟩
-          intro q qdef
-          dsimp [nondomi, domi]
-          intro con
-          simp_rw [Nat.le_zero] at con
-          apply gain.2
-          convert qdef
-          · exact con.1.symm
-          · exact con.2.symm
-      obtain ⟨act, act_mem, act_nz⟩ := this
-      use act
-      constructor
-      · exact (Chomp_state_sub_ini _ _) act_mem
-      · rename_i facts
-        apply Chomp_hist_mem_ini_of_Hist_legal height length _ facts.1 _ hist_leg
-        contrapose! q
-        cases' hist with x l
-        · apply q
-        · apply Chomp_state_zero_act_non_zero _ facts.1 l x q
-          intro con
-          rw [con] at facts
-          apply facts.2
-          exact List.mem_cons_self (0, 0) l
-      · rename_i facts
-        apply Chomp_hist_pairwise_nondomi_of_Hist_legal height length _ facts.1 _ hist_leg
-        contrapose! q
-        cases' hist with x l
-        · apply q
-        · apply Chomp_state_zero_act_non_zero _ facts.1 l x q
-          intro con
-          rw [con] at facts
-          apply facts.2
-          exact List.mem_cons_self (0, 0) l
-      · dsimp [Chomp_state] at act_mem
-        rw [Finset.mem_filter] at act_mem
-        exact act_mem.2
-      · exact act_nz
-    · use (0,0)
-  · simp_rw [if_neg q]
-    use (1,0)
-    split_ifs
-    · decide
-
---#exit
-
-def Chomp (height length : ℕ) : zSymm_Game_World (Finset (ℕ × ℕ)) (ℕ × ℕ) where
-  toSymm_Game_World := preChomp height length
-  law_careless := preChomp_law_careless height length
-  transition_careless := preChomp_tranistion_careless height length
-  coherent := preChomp_coherent height length
-  playable := preChomp_playable height length
-
-
-
-lemma Chomp_state_ini_not_zero (height length : ℕ) (h : height ≠ 0 ∨ length ≠ 0)  : ¬Chomp_state (Chomp_init height length) [] = {(0, 0)} :=
-  by
-  dsimp [Chomp_state, Chomp_init]
-  apply ne_of_not_subset
-  intro con
-  specialize @con (length, height)
-    (by rw [Finset.mem_filter ]
-        constructor
-        · simp_rw [Finset.mem_product, Finset.mem_range]
-          constructor <;> {exact Nat.le.refl}
-        · intro q no ; contradiction)
-  simp only [Finset.mem_singleton, Prod.mk.injEq] at con
-  cases' h with h h
-  · exact h con.2
-  · exact h con.1
-
-
-
-lemma preChomp_law_prop_transition (height length : ℕ) (h : height ≠ 0 ∨ length ≠ 0) (act : ℕ × ℕ) (hist : List (ℕ × ℕ))
-  (leg : Symm_Game_World.law (Chomp height length).toSymm_Game_World (Chomp height length).toSymm_Game_World.init_game_state hist act) :
-  Symm_Game_World.transition (Chomp height length).toSymm_Game_World
-    (Chomp height length).toSymm_Game_World.init_game_state hist act =
-  Symm_Game_World.transition (Chomp height length).toSymm_Game_World
-    (Chomp height length).toSymm_Game_World.init_game_state (hist ++ [(length, height)]) act :=
-  by
-  dsimp [Chomp, preChomp] at *
-  by_cases q1 : (0, 0) ∉ hist
-  · rw [if_pos ⟨Chomp_init_has_zero height length, q1⟩] at leg
-    by_cases q2 : ¬Chomp_state (Chomp_init height length) hist = {(0, 0)}
-    · rw [if_pos q2] at *
-      have hyp : Chomp_state (Chomp_init height length) (act :: hist) = Chomp_state (Chomp_init height length) (act :: (hist ++ [(length, height)])) :=
-        by
-        dsimp [Chomp_state]
-        apply Finset.filter_congr
-        intro x _
-        simp_rw [← List.cons_append, List.mem_append]
-        constructor
-        · intro ca
-          rintro q (qdef | qdef)
-          · exact ca _ qdef
-          · rw [List.mem_singleton] at qdef
-            rw [qdef]
-            specialize ca act (by apply List.mem_cons_self)
-            dsimp [nondomi, domi] at *
-            contrapose! ca
-            constructor
-            · apply le_trans _ ca.1
-              have := leg.act_mem
-              dsimp [Chomp_init] at this
-              rw [Finset.mem_product, Finset.mem_range, Nat.lt_add_one_iff] at this
-              exact this.1
-            · apply le_trans _ ca.2
-              have := leg.act_mem
-              dsimp [Chomp_init] at this
-              simp_rw [Finset.mem_product, Finset.mem_range, Nat.lt_add_one_iff] at this
-              exact this.2
-        · intro ca
-          intro q qdef
-          exact ca _ (Or.inl (qdef))
-      by_cases q3 : ¬Chomp_state (Chomp_init height length) (hist ++ [(length, height)]) = {(0, 0)}
-      · rw [if_pos q3] at *
-        exact hyp
-      · rw [if_neg q3]
-        rw [not_not] at q3
-        rw [hyp]
-        dsimp [Chomp_state] at *
-        ext x
-        constructor
-        · intro xdef
-          rw [← q3]
-          simp_rw [Finset.mem_filter, List.mem_cons] at *
-          refine' ⟨xdef.1, _ ⟩
-          intro q qdef
-          apply xdef.2
-          exact Or.inr qdef
-        · intro xdef
-          rw [Finset.mem_singleton] at xdef
-          rw [xdef]
-          simp_rw [Finset.mem_filter, List.mem_cons]
-          refine' ⟨(Chomp_init_has_zero height length), _ ⟩
-          rintro q (qdef | qdef)
-          · dsimp [nondomi, domi]
-            intro con
-            simp_rw [Nat.le_zero] at con
-            apply leg.nz_act
-            rw [← qdef]
-            ext
-            · exact con.1
-            · exact con.2
-          · rw [Finset.ext_iff] at q3
-            replace q3 := (q3 (0,0)).mpr (by apply Finset.mem_singleton_self)
-            rw [Finset.mem_filter] at q3
-            exact q3.2 _ qdef
-    · rw [if_neg q2] at *
-      rw [not_not] at q2
-      split_ifs with H
-      · rfl
-      · have := Chomp_state_sub (Chomp_init height length) hist [(length, height)]
-        have that : Chomp_state (Chomp_init height length) (hist ++ [(length, height)]) ≠ Chomp_state (Chomp_init height length) hist := by rw [q2] ; exact H
-        have thus := Finset.ssubset_iff_subset_ne.mpr ⟨this,that⟩
-        rw [q2, Finset.ssubset_singleton_iff] at thus
-        have thut := Chomp_state_state_empty _ (Chomp_init_has_zero height length) _ thus
-        rw [List.mem_append] at thut
-        cases' thut with no neither
-        · exact False.elim (q1 no)
-        · rw [List.mem_singleton, Prod.eq_iff_fst_eq_snd_eq] at neither
-          cases' h with h h
-          · exact False.elim (h neither.2.symm)
-          · exact False.elim (h neither.1.symm)
-  · push_neg at q1
-    rw [Chomp_state_hist_zero _ hist q1]
-    rw [Chomp_state_hist_zero _ (act :: hist) (List.mem_cons_of_mem _ q1)]
-    rw [Chomp_state_hist_zero _ (hist ++ [(length, height)]) (List.mem_append_left _ q1)]
-    rw [Chomp_state_hist_zero _ (act ::(hist ++ [(length, height)])) (List.mem_cons_of_mem _ (List.mem_append_left _ q1))]
 
 
 private lemma helper (height length : ℕ) (h : height ≠ 0 ∨ length ≠ 0) : (0,0) ∉ [(length, height)] :=
@@ -1036,296 +183,6 @@ lemma Chomp_init_has_len_hei (height length : ℕ) : (length, height) ∈ Chomp_
   constructor
   all_goals {apply Nat.lt_succ_self}
 
---#exit
-
-lemma preChomp_law_prop_law (height length : ℕ) (h : height ≠ 0 ∨ length ≠ 0) (act : ℕ × ℕ) (hist : List (ℕ × ℕ)) (hh : hist ≠ [])
-  (hh2 : (length, height) ∉ hist)
-  (leg : Symm_Game_World.law (Chomp height length).toSymm_Game_World (Chomp height length).toSymm_Game_World.init_game_state hist act) :
-  Symm_Game_World.law (Chomp height length).toSymm_Game_World (Chomp height length).toSymm_Game_World.init_game_state
-  (hist ++ [(length, height)]) act :=
-  by
-  dsimp [Chomp, preChomp] at *
-  by_cases q0 : (0, 0) ∉ hist
-  · rw [if_pos ⟨Chomp_init_has_zero height length, q0 ⟩ ] at leg
-    rw [if_pos _]
-    swap
-    · refine' ⟨Chomp_init_has_zero height length, _⟩
-      apply List.not_mem_append q0
-      intro con
-      rw [List.mem_singleton, Prod.eq_iff_fst_eq_snd_eq] at con
-      cases' h with h h
-      · exact False.elim (h con.2.symm)
-      · exact False.elim (h con.1.symm)
-    · by_cases q1 : ¬Chomp_state (Chomp_init height length) hist = {(0, 0)}
-      · rw [if_pos q1] at leg
-        by_cases q2 : ¬Chomp_state (Chomp_init height length) (hist ++ [(length, height)]) = {(0, 0)}
-        · rw [if_pos q2]
-          constructor
-          · exact leg.act_mem
-          · intro q qdef
-            rw [List.mem_append] at qdef
-            cases' qdef with qdef qdef
-            · exact leg.hist_mem q qdef
-            · rw [List.mem_singleton] at qdef
-              rw [qdef]
-              apply Chomp_init_has_len_hei
-          · rw [List.pairwise_append]
-            constructor
-            · apply leg.hist_nd
-            · constructor
-              · apply List.pairwise_singleton
-              · intro a ah b bs
-                rw [List.mem_singleton] at bs
-                rw [bs]
-                have ahh := leg.hist_mem a ah
-                dsimp [Chomp_init] at ahh
-                simp_rw [Finset.mem_product, Finset.mem_range, Nat.lt_succ] at ahh
-                intro con
-                dsimp [domi] at con
-                apply hh2
-                convert ah
-                · exact le_antisymm con.1 ahh.1
-                · exact le_antisymm con.2 ahh.2
-          · intro q qdef
-            rw [List.mem_append] at qdef
-            cases' qdef with qdef qdef
-            · exact leg.nd _ qdef
-            · rw [List.mem_singleton] at qdef
-              rw [qdef]
-              dsimp [nondomi, domi]
-              cases' hist with x hist
-              · contradiction
-              · have leg1 := leg.act_mem
-                have leg3 := leg.hist_mem x (by exact List.mem_cons_self x hist)
-                dsimp [Chomp_init] at leg1 leg3
-                simp_rw [Finset.mem_product, Finset.mem_range, Nat.lt_add_one_iff] at leg1 leg3
-                have leg2 := leg.nd x (List.mem_cons_self x hist)
-                dsimp [nondomi, domi] at leg2
-                intro con
-                have uno : act.1 = length := le_antisymm leg1.1 con.1
-                have dos : act.2 = height := le_antisymm leg1.2 con.2
-                rw [← uno, ← dos] at leg3
-                exact leg2 leg3
-          · exact leg.nz_act
-        · rw [if_neg q2]
-          exact leg.nz_act
-      · rw [if_neg q1] at leg
-        rw [not_not] at q1
-        rw [if_neg ]
-        · exact leg
-        · rw [not_not]
-          rw [Finset.eq_singleton_iff_unique_mem]
-          constructor
-          · rw [Chomp_state_has_zero_iff_hist_has_zero]
-            · apply List.not_mem_append q0
-              exact helper _ _ h
-            · apply Chomp_init_has_zero
-          · intro x xdef
-            replace xdef := Chomp_state_sub _ _ _ xdef
-            rw [q1] at xdef
-            rw [Finset.mem_singleton] at xdef
-            exact xdef
-  · rw [not_not] at q0
-    rw [if_neg (by rw [not_and_or] ; right ; rw [not_not] ; exact q0)] at leg
-    rw [if_neg (by rw [not_and_or] ; right ; rw [not_not] ; exact List.mem_append.mpr (Or.inl q0))]
-    trivial
-
-
-
-
-lemma Chomp_History_no_zero (height length : ℕ)  (f_strat s_strat : Strategy (Finset (ℕ × ℕ)) (ℕ × ℕ))
-  (f_leg : Strategy_legal_fst (Chomp height length).init_game_state (Chomp height length).law f_strat s_strat)
-  (s_leg : Strategy_legal_snd (Chomp height length).init_game_state (Chomp height length).law f_strat s_strat)
-  : ∀ t, (0,0) ∉ History_on_turn (Chomp_init height length) f_strat s_strat t :=
-  by
-  intro t
-  induction' t with t ih
-  · dsimp [History_on_turn]
-    trivial
-  · dsimp [History_on_turn]
-    split_ifs with q
-    · apply List.not_mem_cons_of_ne_of_not_mem _ ih
-      specialize f_leg t q
-      dsimp [Chomp, preChomp] at f_leg
-      rw [if_pos ⟨(Chomp_init_has_zero height length), ih⟩] at f_leg
-      split_ifs at f_leg with q2
-      · contrapose! f_leg
-        exact f_leg.symm
-      · intro con
-        apply f_leg.nz_act con.symm
-    · apply List.not_mem_cons_of_ne_of_not_mem _ ih
-      rw [Turn_not_fst_iff_snd] at q
-      specialize s_leg t q
-      dsimp [Chomp, preChomp] at s_leg
-      rw [if_pos ⟨(Chomp_init_has_zero height length), ih⟩] at s_leg
-      split_ifs at s_leg with q2
-      · contrapose! s_leg
-        exact s_leg.symm
-      · intro con
-        apply s_leg.nz_act con.symm
-
-
-
-
-lemma Chomp_strat_non_zero_fst (height length : ℕ) (f_strat s_strat : Strategy (Finset (ℕ × ℕ)) (ℕ × ℕ))
-  (f_leg : Strategy_legal_fst (Chomp height length).init_game_state (Chomp height length).law f_strat s_strat)
-  (s_leg : Strategy_legal_snd (Chomp height length).init_game_state (Chomp height length).law f_strat s_strat) :
-  ∀ t, Turn_fst (t+1) → f_strat (Chomp height length).init_game_state (History_on_turn (Chomp height length).init_game_state f_strat s_strat t) ≠ (0,0) :=
-  by
-  intro t tf
-  have := f_leg t tf
-  dsimp [Chomp, preChomp] at this
-  rw [if_pos ⟨(Chomp_init_has_zero height length), (Chomp_History_no_zero _ _ _ _ f_leg s_leg  t)⟩] at this
-  split_ifs at this with q2
-  · exact this
-  · intro con
-    apply this.nz_act con
-
-
-lemma Chomp_strat_non_zero_snd (height length : ℕ) (f_strat s_strat : Strategy (Finset (ℕ × ℕ)) (ℕ × ℕ))
-  (f_leg : Strategy_legal_fst (Chomp height length).init_game_state (Chomp height length).law f_strat s_strat)
-  (s_leg : Strategy_legal_snd (Chomp height length).init_game_state (Chomp height length).law f_strat s_strat) :
-  ∀ t, Turn_snd (t+1) → s_strat (Chomp height length).init_game_state (History_on_turn (Chomp height length).init_game_state f_strat s_strat t) ≠ (0,0) :=
-  by
-  intro t tf
-  have := s_leg t tf
-  dsimp [Chomp, preChomp] at this
-  rw [if_pos ⟨(Chomp_init_has_zero height length), (Chomp_History_no_zero _ _ _ _ f_leg s_leg  t)⟩] at this
-  split_ifs at this with q2
-  · exact this
-  · intro con
-    apply this.nz_act con
-
-
-
-
-lemma Chomp_state_on_turn_has_zero (height length : ℕ)  (f_strat s_strat : Strategy (Finset (ℕ × ℕ)) (ℕ × ℕ))
-  (f_leg : Strategy_legal_fst (Chomp height length).init_game_state (Chomp height length).law f_strat s_strat)
-  (s_leg : Strategy_legal_snd (Chomp height length).init_game_state (Chomp height length).law f_strat s_strat)
-  :
-  ∀ t, (0,0) ∈ (Chomp height length).state_on_turn f_strat s_strat t :=
-  by
-  intro t
-  cases' t with t
-  · dsimp [Symm_Game_World.state_on_turn]
-    dsimp [Chomp, preChomp, Symm_Game_World.history_on_turn, History_on_turn]
-    apply Chomp_init_has_zero
-  · dsimp [Symm_Game_World.state_on_turn]
-    by_cases q : Turn_fst (t + 1)
-    · rw [if_pos q]
-      dsimp [Chomp, preChomp]
-      by_cases q1 : Chomp_state (Chomp_init height length) ((Chomp height length).history_on_turn f_strat s_strat t) = {(0,0)}
-      · rw [if_neg (by rw [not_not] ; apply q1)]
-        exact Finset.mem_singleton.mpr rfl
-      · rw [if_pos (by apply q1)]
-        rw [Chomp_state_has_zero_iff_hist_has_zero _ (by apply Chomp_init_has_zero)]
-        apply List.not_mem_cons_of_ne_of_not_mem
-        · exact (Chomp_strat_non_zero_fst _ _ _ _ f_leg s_leg t q).symm
-        · apply (Chomp_History_no_zero _ _ _ _ f_leg s_leg  t)
-    · rw [if_neg q]
-      rw [Turn_not_fst_iff_snd] at q
-      dsimp [Chomp, preChomp]
-      by_cases q1 : Chomp_state (Chomp_init height length) ((Chomp height length).history_on_turn f_strat s_strat t) = {(0,0)}
-      · rw [if_neg (by rw [not_not] ; apply q1)]
-        exact Finset.mem_singleton.mpr rfl
-      · rw [if_pos (by apply q1)]
-        rw [Chomp_state_has_zero_iff_hist_has_zero _ (by apply Chomp_init_has_zero)]
-        apply List.not_mem_cons_of_ne_of_not_mem
-        · exact (Chomp_strat_non_zero_snd _ _ _ _ f_leg s_leg t q).symm
-        · apply (Chomp_History_no_zero _ _ _ _ f_leg s_leg  t)
-
-
-
-
-
-lemma Chomp_state_on_turn_sub (height length : ℕ) (h : height ≠ 0 ∨ length ≠ 0) (f_strat s_strat : Strategy (Finset (ℕ × ℕ)) (ℕ × ℕ))
-  (f_leg : Strategy_legal_fst (Chomp height length).init_game_state (Chomp height length).law f_strat s_strat)
-  (s_leg : Strategy_legal_snd (Chomp height length).init_game_state (Chomp height length).law f_strat s_strat)
-  :
-  ∀ t, ((Chomp height length).state_on_turn f_strat s_strat (t+1)) ⊆ (Chomp height length).state_on_turn f_strat s_strat t :=
-  by
-  intro t
-  cases' t with t
-  · dsimp [Symm_Game_World.state_on_turn]
-    rw [if_pos (by decide)]
-    dsimp [Chomp, preChomp, Symm_Game_World.history_on_turn, History_on_turn]
-    rw [if_pos (by apply Chomp_state_ini_not_zero _ _ h)]
-    apply Chomp_state_sub_ini
-  · dsimp [Symm_Game_World.state_on_turn]
-    by_cases q : Turn_fst (t + 1)
-    · rw [if_pos q]
-      rw [Turn_fst_not_step] at q
-      rw [if_neg q]
-      dsimp [Chomp, preChomp]
-      rw [← Turn_fst_not_step] at q
-      by_cases q1 : Chomp_state (Chomp_init height length) ((Chomp height length).history_on_turn f_strat s_strat t) = {(0,0)}
-      · have : Chomp_state (Chomp_init height length) ((Chomp height length).history_on_turn f_strat s_strat (t+1)) = {(0,0)} :=
-          by
-          dsimp [Symm_Game_World.history_on_turn, History_on_turn]
-          rw [if_pos q]
-          apply Chomp_state_zero_act_non_zero
-          · apply Chomp_init_has_zero
-          · exact q1
-          · apply Chomp_strat_non_zero_fst _ _ _ _ f_leg s_leg t q
-        rw [if_neg (by rw [not_not] ; apply this), if_neg (by rw [not_not] ; apply q1)]
-      · by_cases q2 : Chomp_state (Chomp_init height length) ((Chomp height length).history_on_turn f_strat s_strat (t+1)) = {(0,0)}
-        · rw [if_neg (by rw [not_not]; apply q2)]
-          rw [if_pos (by apply q1)]
-          rw [Finset.singleton_subset_iff]
-          rw [Chomp_state_has_zero_iff_hist_has_zero _ (by apply Chomp_init_has_zero)]
-          apply List.not_mem_cons_of_ne_of_not_mem
-          · exact (Chomp_strat_non_zero_fst _ _ _ _ f_leg s_leg t q).symm
-          · apply (Chomp_History_no_zero _ _ _ _ f_leg s_leg  t)
-        · rw [if_pos (by apply q2)]
-          rw [if_pos (by apply q1)]
-          apply Chomp_state_sub_of_hist_sub
-          dsimp [Symm_Game_World.history_on_turn, History_on_turn]
-          rw [if_pos q]
-          exact fun ⦃a⦄ a_1 =>
-            List.Mem.tail
-              (s_strat (Chomp_init height length)
-                (f_strat (Chomp_init height length)
-                    (History_on_turn (Chomp_init height length) f_strat s_strat t) ::
-                  History_on_turn (Chomp_init height length) f_strat s_strat t))
-              a_1
-    · rw [if_neg q]
-      rw [Turn_fst_not_step, not_not] at q
-      rw [if_pos q]
-      dsimp [Chomp, preChomp]
-      replace q := not_not.mpr q -- rw fails, pathetic
-      rw [← Turn_fst_not_step] at q
-      by_cases q1 : Chomp_state (Chomp_init height length) ((Chomp height length).history_on_turn f_strat s_strat t) = {(0,0)}
-      · have : Chomp_state (Chomp_init height length) ((Chomp height length).history_on_turn f_strat s_strat (t+1)) = {(0,0)} :=
-          by
-          dsimp [Symm_Game_World.history_on_turn, History_on_turn]
-          rw [if_neg q]
-          apply Chomp_state_zero_act_non_zero
-          · apply Chomp_init_has_zero
-          · exact q1
-          · apply Chomp_strat_non_zero_snd _ _ _ _ f_leg s_leg t q
-        rw [if_neg (by rw [not_not] ; apply this), if_neg (by rw [not_not] ; apply q1)]
-      · by_cases q2 : Chomp_state (Chomp_init height length) ((Chomp height length).history_on_turn f_strat s_strat (t+1)) = {(0,0)}
-        · rw [if_neg (by rw [not_not]; apply q2)]
-          rw [if_pos (by apply q1)]
-          rw [Finset.singleton_subset_iff]
-          rw [Chomp_state_has_zero_iff_hist_has_zero _ (by apply Chomp_init_has_zero)]
-          apply List.not_mem_cons_of_ne_of_not_mem
-          · exact (Chomp_strat_non_zero_snd _ _ _ _ f_leg s_leg t q).symm
-          · apply (Chomp_History_no_zero _ _ _ _ f_leg s_leg  t)
-        · rw [if_pos (by apply q2)]
-          rw [if_pos (by apply q1)]
-          apply Chomp_state_sub_of_hist_sub
-          dsimp [Symm_Game_World.history_on_turn, History_on_turn]
-          rw [if_neg q]
-          exact fun ⦃a⦄ a_1 =>
-            List.Mem.tail
-              (f_strat (Chomp_init height length)
-                (s_strat (Chomp_init height length)
-                    (History_on_turn (Chomp_init height length) f_strat s_strat t) ::
-                  History_on_turn (Chomp_init height length) f_strat s_strat t))
-              a_1
-
-
 lemma Chomp_state_empty  (ini : (Finset (ℕ × ℕ))) : Chomp_state ini [] = ini :=
   by
   dsimp [Chomp_state]
@@ -1344,334 +201,387 @@ lemma Chomp_not_mem_state_of_mem_hist (ini : (Finset (ℕ × ℕ))) (hist : (Lis
   exact ⟨le_refl act.1, le_refl act.2⟩
 
 
-lemma Chomp_state_eq_state_on_turn (height length : ℕ) (f_strat s_strat : Strategy (Finset (ℕ × ℕ)) (ℕ × ℕ))
-  (f_leg : Strategy_legal_fst (Chomp height length).init_game_state (Chomp height length).law f_strat s_strat)
-  (s_leg : Strategy_legal_snd (Chomp height length).init_game_state (Chomp height length).law f_strat s_strat)
-  (t : ℕ) :
-  (Chomp height length).state_on_turn f_strat s_strat t = Chomp_state (Chomp height length).init_game_state (History_on_turn (Chomp height length).init_game_state f_strat s_strat t) :=
-  by
-  cases' t with t
-  · dsimp [Symm_Game_World.state_on_turn, History_on_turn]
-    rw [Chomp_state_empty]
-  · dsimp [Symm_Game_World.state_on_turn, History_on_turn]
-    by_cases q : Turn_fst (t + 1)
-    · simp_rw [if_pos q]
-      dsimp [Chomp, preChomp]
-      split_ifs with q2
-      · dsimp [Symm_Game_World.history_on_turn] at q2
-        rw [eq_comm]
-        apply Chomp_state_zero_act_non_zero
-        · apply Chomp_init_has_zero
-        · exact q2
-        · apply Chomp_strat_non_zero_fst _ _ _ _ f_leg s_leg t q
-      · rfl
-    · simp_rw [if_neg q]
-      dsimp [Chomp, preChomp]
-      split_ifs with q2
-      · dsimp [Symm_Game_World.history_on_turn] at q2
-        rw [eq_comm]
-        apply Chomp_state_zero_act_non_zero
-        · apply Chomp_init_has_zero
-        · exact q2
-        · apply Chomp_strat_non_zero_snd _ _ _ _ f_leg s_leg t q
-      · rfl
 
-lemma Chomp_act_mem_state_of_law (ini : (Finset (ℕ × ℕ))) (hist : (List (ℕ × ℕ))) (act : ℕ × ℕ) (leg : Chomp_law ini hist act) :
-  act ∈ Chomp_state ini hist :=
-  by
-  dsimp [Chomp_state]
-  rw [Finset.mem_filter]
-  exact ⟨leg.act_mem, leg.nd ⟩
+
+-- # Chomp law lemmata
+
+
+/--
+Selecting a tile `act` is legal, if it was in the initial board,
+and it isn't dominated by one of the tiles played sofar.
+-/
+structure Chomp_law (ini : Finset (ℕ × ℕ)) (hist : List (ℕ × ℕ)) (act : ℕ × ℕ) : Prop where
+  act_mem : act ∈ ini
+  nd : ∀ q ∈ hist, nondomi q act
 
 
 
 
-lemma Chomp_state_cons_eq (ini : (Finset (ℕ × ℕ))) (hist : (List (ℕ × ℕ))) (act : ℕ × ℕ)
-  (main : Chomp_state ini (act :: hist) = Chomp_state ini hist) :
-  ¬ Chomp_law ini hist act :=
-  by
-  intro con
-  replace con := Chomp_act_mem_state_of_law _ _ _ con
-  rw [← main] at con
-  dsimp [Chomp_state] at con
-  rw [Finset.mem_filter] at con
-  replace con := con.2 act (by exact List.mem_cons_self act hist)
-  apply con
-  exact ⟨le_refl act.1, le_refl act.2⟩
+
+-- # Chomp win states lemmata
+
+/--
+A terminal position is reached when playing `final_a` at history `final_h`,
+if the board wasn't empty at that history, but is after playing the move.
+To have a coherent end for this game, all histories extending such a history
+are also considered terminal.
+-/
+structure Chomp_win_final (ini : Finset (ℕ × ℕ)) (hist final_h : List (ℕ × ℕ)) (final_a : ℕ × ℕ) : Prop where
+  N : Chomp_state ini final_h ≠ ∅
+  F : Chomp_state ini (final_a :: final_h) = ∅
+  ref : (final_a :: final_h) <:+ hist
+
+/--
+The game is won by the frist player if the terminal position was reached on the second turn.
+-/
+def Chomp_win_fst (ini : Finset (ℕ × ℕ)) (hist : List (ℕ × ℕ)) : Prop :=
+  ∃ final_h : List (ℕ × ℕ), ∃ final_a : (ℕ × ℕ), Turn_snd (final_h.length + 1) ∧ Chomp_win_final ini hist final_h final_a
+
+/--
+The game is won by the second player if the terminal position was reached on the first turn.
+-/
+def Chomp_win_snd (ini : Finset (ℕ × ℕ)) (hist : List (ℕ × ℕ)) : Prop :=
+  ∃ final_h : List (ℕ × ℕ), ∃ final_a : (ℕ × ℕ), Turn_fst (final_h.length + 1) ∧ Chomp_win_final ini hist final_h final_a
+
+
+lemma Chomp_win_final_ext (ini : Finset (ℕ × ℕ)) (hist final_h : List (ℕ × ℕ)) (final_a act: ℕ × ℕ) :
+  Chomp_win_final ini hist final_h final_a → Chomp_win_final ini (act :: hist) final_h final_a := by
+  intro main
+  constructor
+  · exact main.N
+  · exact main.F
+  · apply List.IsSuffix.trans main.ref
+    exact List.suffix_cons act hist
+
+lemma Chomp_win_fst_ext (ini : Finset (ℕ × ℕ)) (hist : List (ℕ × ℕ)) (act: ℕ × ℕ) :
+  Chomp_win_fst ini hist → Chomp_win_fst ini (act :: hist) := by
+  rintro ⟨h, a, t, p⟩
+  exact ⟨h,a,t, Chomp_win_final_ext ini hist h a act p⟩
+
+lemma Chomp_win_snd_ext (ini : Finset (ℕ × ℕ)) (hist : List (ℕ × ℕ)) (act: ℕ × ℕ) :
+  Chomp_win_snd ini hist → Chomp_win_snd ini (act :: hist) := by
+  rintro ⟨h, a, t, p⟩
+  exact ⟨h,a,t, Chomp_win_final_ext ini hist h a act p⟩
 
 
 
---#exit
+-- # preChomp
 
-lemma Chomp_state_on_turn_sub_strict (height length : ℕ) (h : height ≠ 0 ∨ length ≠ 0) (f_strat s_strat : Strategy (Finset (ℕ × ℕ)) (ℕ × ℕ))
-  (f_leg : Strategy_legal_fst (Chomp height length).init_game_state (Chomp height length).law f_strat s_strat)
-  (s_leg : Strategy_legal_snd (Chomp height length).init_game_state (Chomp height length).law f_strat s_strat)
-  (t : ℕ) (hs : (Chomp height length).state_on_turn f_strat s_strat t ≠ {(0,0)}):
-  ((Chomp height length).state_on_turn f_strat s_strat (t+1)) ⊂ (Chomp height length).state_on_turn f_strat s_strat t :=
-  by
-  rw [Finset.ssubset_iff_subset_ne]
-  refine' ⟨Chomp_state_on_turn_sub _ _ h _ _ f_leg s_leg t, _ ⟩
-  intro con
-  simp_rw [Chomp_state_eq_state_on_turn _ _ _ _ f_leg s_leg] at *
-  dsimp [History_on_turn] at con
-  by_cases q : Turn_fst (t + 1)
-  · rw [if_pos q] at con
-    have := f_leg t q
-    dsimp [Chomp, preChomp] at this
-    rw [if_pos ⟨Chomp_init_has_zero _ _ , Chomp_History_no_zero _ _ _ _ f_leg s_leg  t⟩] at this
-    rw [if_pos (by apply hs)] at this
-    replace con := Chomp_state_cons_eq _ _ _ con
-    exact con this
-  · rw [if_neg q] at con
-    have := s_leg t q
-    dsimp [Chomp, preChomp] at this
-    rw [if_pos ⟨Chomp_init_has_zero _ _ , Chomp_History_no_zero _ _ _ _ f_leg s_leg  t⟩] at this
-    rw [if_pos (by apply hs)] at this
-    replace con := Chomp_state_cons_eq _ _ _ con
-    exact con this
 
-lemma Chomp_state_zero_stays (height length : ℕ) (h : height ≠ 0 ∨ length ≠ 0) (f_strat s_strat : Strategy (Finset (ℕ × ℕ)) (ℕ × ℕ))
-  (f_leg : Strategy_legal_fst (Chomp height length).init_game_state (Chomp height length).law f_strat s_strat)
-  (s_leg : Strategy_legal_snd (Chomp height length).init_game_state (Chomp height length).law f_strat s_strat)
-  (t : ℕ) (hs : (Chomp height length).state_on_turn f_strat s_strat t = {(0,0)}) :
-  (Chomp height length).state_on_turn f_strat s_strat (t + 1) = {(0,0)} :=
-  by
-  rw [Finset.eq_singleton_iff_unique_mem]
-  refine' ⟨Chomp_state_on_turn_has_zero _ _ _ _ f_leg s_leg (t+1), _ ⟩
-  intro x xdef
-  replace xdef := (Chomp_state_on_turn_sub _ _ h _ _ f_leg s_leg t) xdef
-  rw [hs, Finset.mem_singleton] at xdef
-  exact xdef
+def preChomp (height length : ℕ) : Symm_Game_World (Finset (ℕ × ℕ)) (ℕ × ℕ) where
+  init_game_state := Chomp_init height length
+  fst_win_states := fun hist => Chomp_win_fst (Chomp_init height length) hist
+  snd_win_states := fun hist => Chomp_win_snd (Chomp_init height length) hist
+  transition := fun hist act => Chomp_state (Chomp_init height length) (act :: hist)
+  law := fun hist act =>  if Chomp_state (Chomp_init height length) hist ≠ ∅
+                          then Chomp_law (Chomp_init height length) hist act
+                          else True
 
 
 
-lemma Chomp_state_zero_stays_strong (height length : ℕ) (h : height ≠ 0 ∨ length ≠ 0) (f_strat s_strat : Strategy (Finset (ℕ × ℕ)) (ℕ × ℕ))
-  (f_leg : Strategy_legal_fst (Chomp height length).init_game_state (Chomp height length).law f_strat s_strat)
-  (s_leg : Strategy_legal_snd (Chomp height length).init_game_state (Chomp height length).law f_strat s_strat)
-  (t : ℕ) (hs : (Chomp height length).state_on_turn f_strat s_strat t = {(0,0)}) :
-  ∀ n, (Chomp height length).state_on_turn f_strat s_strat (t + n) = {(0,0)} :=
-  by
-  intro n
-  induction' n with n ih
-  · exact hs
-  · rw [Nat.add_succ]
-    apply Chomp_state_zero_stays  _ _ h _ _ f_leg s_leg (t+n) ih
+-- # Chomp is WL
 
 
-lemma Chomp_WLT (height length : ℕ) (h : height ≠ 0 ∨ length ≠ 0) : (Chomp height length).isWL_wBound ((length +1) * (height + 1)) :=
-  by
-  intro f_strat s_strat f_leg s_leg
-  use ((length +1) * (height + 1))
-  refine' ⟨le_refl ((length +1) * (height + 1)), _ ⟩
-  dsimp [Symm_Game_World.Turn_isWL, Chomp, preChomp]
-  by_contra! con
-  have dec : ∀ t ≤ ((length +1) * (height + 1)), (Symm_Game_World.state_on_turn (Chomp height length).toSymm_Game_World f_strat s_strat t).card ≤ ((length +1) * (height + 1)) - t :=
+lemma preChomp_state_sub {height length : ℕ}
+  (f_strat : (preChomp height length).fStrategy) (s_strat : (preChomp height length).sStrategy) :
+  ∀  n,  Chomp_state (preChomp height length).init_game_state ((preChomp height length).hist_on_turn f_strat s_strat (n+1))
+    ⊆ Chomp_state (preChomp height length).init_game_state ((preChomp height length).hist_on_turn f_strat s_strat (n)) :=
     by
-    intro t tdef
-    have : ∀ t ≤ ((length +1) * (height + 1)), (Symm_Game_World.state_on_turn (Chomp height length).toSymm_Game_World f_strat s_strat t) ≠  {(0,0)} :=
-      by
-      intro n ndef con'
-      have := Chomp_state_zero_stays_strong _ _ h _ _ f_leg s_leg n con' (((length +1) * (height + 1)) - n)
-      rw [Nat.add_sub_cancel' ndef] at this
-      exact con this
-    induction' t with t ih
-    · dsimp [Symm_Game_World.state_on_turn, Chomp, preChomp, Chomp_init]
-      simp_rw [Finset.card_product, Finset.card_range]
-      apply le_refl
-    · have that := Finset.card_lt_card ((Chomp_state_on_turn_sub_strict _ _ h _ _ f_leg s_leg t) (this t (by apply le_trans _ tdef ; apply Nat.le_succ )))
-      rw [Nat.lt_iff_add_one_le] at that
-      rw [Nat.sub_succ', Nat.le_sub_iff_add_le (by rw [Nat.le_sub_iff_add_le, add_comm] ; apply tdef ; apply le_trans _ tdef ; apply Nat.le_succ)]
-      exact le_trans that (ih (by apply le_trans _ tdef ; apply Nat.le_succ ))
-  specialize dec ((length +1) * (height + 1)) (le_refl _)
-  rw [Nat.sub_self, Nat.le_zero, Finset.card_eq_zero] at dec
-  apply Finset.not_mem_empty (0,0)
-  rw [← dec]
-  apply Chomp_state_on_turn_has_zero _ _ _ _ f_leg s_leg
+    intro n
+    dsimp [Symm_Game_World.hist_on_turn, Game_World.hist_on_turn]
+    split_ifs with T
+    · dsimp
+      apply Chomp_state_sub_cons
+    · dsimp
+      apply Chomp_state_sub_cons
 
 
 
+lemma preChomp_state_ssub {height length : ℕ}
+  (f_strat : (preChomp height length).fStrategy)
+  (s_strat : (preChomp height length).sStrategy) :
+  ∀  n,  Chomp_state (preChomp height length).init_game_state ((preChomp height length).hist_on_turn f_strat s_strat (n)) ≠ ∅ →
+    Chomp_state (preChomp height length).init_game_state ((preChomp height length).hist_on_turn f_strat s_strat (n+1))
+    ⊂ Chomp_state (preChomp height length).init_game_state ((preChomp height length).hist_on_turn f_strat s_strat (n)) :=
+    by
+    intro n hn
+    rw [Finset.ssubset_iff_of_subset (preChomp_state_sub f_strat s_strat n)]
+    dsimp [Symm_Game_World.hist_on_turn, Game_World.hist_on_turn]
+    split_ifs with T
+    · dsimp
+      let act := (f_strat ((preChomp height length).hist_on_turn f_strat s_strat (n)).val (by rw [Symm_Game_World.hist_on_turn_length] ; exact T) ((preChomp height length).hist_on_turn f_strat s_strat (n)).prop.1)
+      use act.val
+      constructor
+      · rw [Chomp_state, Finset.mem_filter]
+        constructor
+        · have := act.prop
+          dsimp [preChomp] at this hn
+          rw [if_pos hn] at this
+          apply this.act_mem
+        · have := act.prop
+          dsimp [preChomp] at this hn
+          rw [if_pos hn] at this
+          apply this.nd
+      · apply Chomp_not_mem_state_of_mem_hist
+        apply List.mem_cons_self
+    · dsimp
+      let act := (s_strat ((preChomp height length).hist_on_turn f_strat s_strat (n)).val (by rw [Symm_Game_World.hist_on_turn_length] ; exact T) ((preChomp height length).hist_on_turn f_strat s_strat (n)).prop.1)
+      use act.val
+      constructor
+      · rw [Chomp_state, Finset.mem_filter]
+        constructor
+        · have := act.prop
+          dsimp [preChomp] at this hn
+          rw [if_pos hn] at this
+          apply this.act_mem
+        · have := act.prop
+          dsimp [preChomp] at this hn
+          rw [if_pos hn] at this
+          apply this.nd
+      · apply Chomp_not_mem_state_of_mem_hist
+        apply List.mem_cons_self
 
-noncomputable
-def stolen_strat
-  (trap : β) (ws : Strategy α β) : Strategy α β :=
-  fun ini hist =>
-    if hist = []
-    then ws ini [trap]
-    else ws ini (hist.dropLast ++ [ws ini [trap] , trap])
 
 
-noncomputable
-def pre_stolen_strat
-  (trap : β) (s_strat : Strategy α β) : Strategy α β :=
-  fun ini hist =>
-    if hist = []
-    then trap
-    else s_strat ini (hist.dropLast)
-
-
-
-lemma History_on_turn_stolen_getLast (ini : α)
-  (trap : β) (ws s_strat : Strategy α β) (t : ℕ) :
-  (History_on_turn ini (stolen_strat trap ws) s_strat (t+1)).getLast (by apply History_on_turn_nonempty_of_succ) = ws ini [trap] :=
+lemma preChomp_reaches_empty {height length : ℕ}
+  (f_strat : (preChomp height length).fStrategy)
+  (s_strat : (preChomp height length).sStrategy) :
+  ∃ n, Chomp_state (preChomp height length).init_game_state ((preChomp height length).hist_on_turn f_strat s_strat (n+1)) = ∅ ∧
+    ∀ m ≤ n, Chomp_state (preChomp height length).init_game_state ((preChomp height length).hist_on_turn f_strat s_strat (m)) ≠ ∅ :=
   by
-  induction' t with t ih
-  · dsimp!
-    unfold stolen_strat
-    rw [if_pos (by rfl)]
-  · dsimp [History_on_turn] at *
-    by_cases q : Turn_fst (Nat.succ t + 1)
-    · simp_rw [if_pos q]
-      rw [List.getLast_cons, ih]
-    · simp_rw [if_neg q]
-      rw [List.getLast_cons, ih]
+  let states := {s | ∃ n, s = Chomp_state (preChomp height length).init_game_state ((preChomp height length).hist_on_turn f_strat s_strat (n)) ∧ s ≠ ∅}
+  have lem : Chomp_state (preChomp height length).init_game_state ((preChomp height length).hist_on_turn f_strat s_strat 0).val ≠ ∅ :=
+    by
+    dsimp only [Symm_Game_World.hist_on_turn, Game_World.hist_on_turn, Chomp_state, preChomp]
+    rw [Finset.filter_true_of_mem]
+    · rw [← Finset.nonempty_iff_ne_empty]
+      use (length, height)
+      apply Chomp_init_has_len_hei height length
+    · intro _ _ _ no
+      contradiction
+  have states_nonempty : Set.Nonempty states := by
+    use  Chomp_state (preChomp height length).init_game_state ((preChomp height length).hist_on_turn f_strat s_strat 0)
+    use 0
+  obtain ⟨n,ndef,ne⟩ := WellFounded.min_mem Finset.isWellFounded_ssubset.wf states states_nonempty
+  use n
+  constructor
+  · by_contra con
+    apply @WellFounded.not_lt_min _ _ Finset.isWellFounded_ssubset.wf states states_nonempty (Chomp_state (preChomp height length).init_game_state ((preChomp height length).hist_on_turn f_strat s_strat (n+1))) (by use n+1)
+    rw [ndef]
+    apply preChomp_state_ssub f_strat s_strat n
+    rw [← ndef]
+    exact ne
+  · intro m mln
+    contrapose ne
+    rw [ndef, not_not, ← Finset.subset_empty]
+    rw [not_not] at ne
+    rw [← ne]
+    apply Chomp_state_sub_of_hist_suffix
+    apply Symm_Game_World.hist_on_turn_suffix
+    exact mln
 
 
-lemma History_on_turn_stolen_pre_stolen (ini : α)
-  (trap : β) (ws s_strat : Strategy α β) (t : ℕ) :
-  (History_on_turn ini (stolen_strat trap ws) s_strat t) ++ [trap] =
-  History_on_turn ini (pre_stolen_strat trap s_strat) ws (t+1) :=
+
+lemma preChomp_isWL (height length : ℕ) : (preChomp height length).isWL :=
   by
-  induction' t with t ih
-  · dsimp [History_on_turn, stolen_strat, pre_stolen_strat]
-    rw [if_pos (by decide), if_pos (by rfl)]
-  · dsimp [History_on_turn]
-    by_cases q : Turn_fst (t + 1)
-    · simp_rw [if_pos q]
-      rw [Turn_fst_not_step] at q
-      rw [if_neg q]
-      rw [List.cons_append, ih]
-      dsimp [History_on_turn]
-      rw [← Turn_fst_not_step] at q
-      rw [if_pos q]
-      congr
-      cases' t with t
-      · dsimp [History_on_turn, stolen_strat, pre_stolen_strat]
-        rw [if_pos (by rfl), if_pos (by rfl)]
-      · unfold stolen_strat
-        rw [if_neg (by apply History_on_turn_nonempty_of_succ)]
-        rw [show [ws ini [trap], trap] = [ws ini [trap]] ++ [trap] from (by simp only [List.singleton_append]) ]
-        rw [← List.append_assoc]
-        have := History_on_turn_stolen_getLast ini trap ws s_strat (t)
-        have that := @List.dropLast_append_getLast _ (History_on_turn ini (stolen_strat trap ws) s_strat (t + 1)) (by apply History_on_turn_nonempty_of_succ)
-        rw [← this]
-        unfold stolen_strat at *
-        rw [that]
-        rw [ih]
-        congr
-        dsimp [History_on_turn]
-        simp_rw [if_pos q]
-    · simp_rw [if_neg q]
-      rw [Turn_fst_not_step, not_not] at q
-      rw [if_pos q]
-      rw [List.cons_append, ih]
-      dsimp [History_on_turn] at *
-      rw [← @not_not (Turn_fst (t + 1 + 1)), ← Turn_fst_not_step] at q
-      simp_rw [if_neg q] at *
-      congr
-      rw [← ih]
-      rw [List.dropLast_append_cons]
-      dsimp
-      rw [List.append_nil]
+  intro f_strat s_strat
+  obtain ⟨T,Tdef⟩ := preChomp_reaches_empty f_strat s_strat
+  use (T+1)
+  by_cases Tt : Turn_fst (T+1)
+  · apply Game_World.Turn_isWL.ws
+    dsimp [preChomp, Chomp_win_snd]
+    use ((preChomp height length).hist_on_turn f_strat s_strat T)
+    use f_strat ((preChomp height length).hist_on_turn f_strat s_strat T).val (by rw [Symm_Game_World.hist_on_turn_length] ; exact Tt) ((preChomp height length).hist_on_turn f_strat s_strat T).prop.1
+    constructor
+    · rw [Symm_Game_World.hist_on_turn_length] ; exact Tt
+    · constructor
+      · apply Tdef.2
+        apply le_refl
+      · convert Tdef.1
+        dsimp [Symm_Game_World.hist_on_turn, Game_World.hist_on_turn]
+        rw [dif_pos Tt]
+      · dsimp [Symm_Game_World.hist_on_turn, Game_World.hist_on_turn]
+        rw [dif_pos Tt]
+        apply List.suffix_refl
+  · apply Game_World.Turn_isWL.wf
+    dsimp [preChomp, Chomp_win_snd]
+    use ((preChomp height length).hist_on_turn f_strat s_strat T)
+    use s_strat ((preChomp height length).hist_on_turn f_strat s_strat T).val (by rw [Symm_Game_World.hist_on_turn_length] ; exact Tt) ((preChomp height length).hist_on_turn f_strat s_strat T).prop.1
+    constructor
+    · rw [Symm_Game_World.hist_on_turn_length] ; exact Tt
+    · constructor
+      · apply Tdef.2
+        apply le_refl
+      · convert Tdef.1
+        dsimp [Symm_Game_World.hist_on_turn, Game_World.hist_on_turn]
+        rw [dif_neg Tt]
+      · dsimp [Symm_Game_World.hist_on_turn, Game_World.hist_on_turn]
+        rw [dif_neg Tt]
+        apply List.suffix_refl
 
 
-lemma Chomp_len_heigh_legal (height length : ℕ) (h : height ≠ 0 ∨ length ≠ 0) :
-  Symm_Game_World.law (Chomp height length).toSymm_Game_World (Chomp height length).toSymm_Game_World.init_game_state [] (length, height) :=
+
+
+
+-- # Chomp is playable
+
+
+lemma preChomp_playable (height length : ℕ) : (preChomp height length).playable :=
+  by
+  intro h _
+  constructor
+  · intro _
+    by_cases q : Chomp_state (Chomp_init height length) h ≠ ∅
+    · dsimp [preChomp]
+      simp_rw [if_pos q]
+      use (0,0)
+      constructor
+      · apply Chomp_init_has_zero
+      · intro x xh
+        rw [nondomi_zero]
+        intro con
+        apply q
+        apply Chomp_state_hist_zero
+        rw [con] at xh
+        exact xh
+    · dsimp [preChomp]
+      simp_rw [if_neg q]
+      use (0,0)
+  · intro _
+    by_cases q : Chomp_state (Chomp_init height length) h ≠ ∅
+    · dsimp [preChomp]
+      simp_rw [if_pos q]
+      use (0,0)
+      constructor
+      · apply Chomp_init_has_zero
+      · intro x xh
+        rw [nondomi_zero]
+        intro con
+        apply q
+        apply Chomp_state_hist_zero
+        rw [con] at xh
+        exact xh
+    · dsimp [preChomp]
+      simp_rw [if_neg q]
+      use (0,0)
+
+
+
+
+-- # Chomp has a coherent end
+
+
+-- to mathlib
+lemma List.suffix_same {a b c : List α} (ha : a <:+ c) (hb : b <:+ c) : a <:+ b ∨ b <:+ a := by
+  induction' c with x l ih
+  · rw [List.suffix_nil] at ha hb
+    rw [ha,hb]
+    simp only [suffix_nil, or_self]
+  · rw [List.suffix_cons_iff] at ha hb
+    cases' ha with ha ha
+    · cases' hb with hb hb
+      · rw [ha,hb]
+        left
+        exact suffix_rfl
+      · rw [ha]
+        right
+        apply IsSuffix.trans hb
+        apply List.suffix_cons
+    · cases' hb with hb hb
+      · rw [hb]
+        left
+        apply IsSuffix.trans ha
+        apply List.suffix_cons
+      · exact ih ha hb
+
+
+lemma preChomp_coherent_end (height length : ℕ) : (preChomp height length).coherent_end :=
+  by
+  constructor
+  · intro h _ con
+    dsimp [preChomp, Chomp_win_fst, Chomp_win_snd] at con
+    obtain ⟨fhs,fas,ts,ws⟩ := con.1
+    obtain ⟨fhf,faf,tf,wf⟩ := con.2
+    cases' List.suffix_same ws.ref wf.ref with q q
+    · rw [List.suffix_cons_iff] at q
+      cases' q with q q
+      · replace q := congrArg List.length q
+        simp_rw [List.length_cons, Nat.succ_inj] at q
+        rw [← q, Turn_fst_iff_not_snd] at tf
+        exact tf ts
+      · have := Chomp_state_sub_of_hist_suffix (Chomp_init height length) _ _ q
+        rw [ws.F, Finset.subset_empty] at this
+        exact wf.N this
+    · rw [List.suffix_cons_iff] at q
+      cases' q with q q
+      · replace q := congrArg List.length q
+        simp_rw [List.length_cons, Nat.succ_inj] at q
+        rw [← q, Turn_snd_iff_not_fst] at ts
+        exact ts tf
+      · have := Chomp_state_sub_of_hist_suffix (Chomp_init height length) _ _ q
+        rw [wf.F, Finset.subset_empty] at this
+        exact ws.N this
+  · intro h _ ws act _
+    apply Chomp_win_fst_ext
+    dsimp [preChomp] at ws
+    exact ws
+  · intro h _ ws act _
+    apply Chomp_win_snd_ext
+    dsimp [preChomp] at ws
+    exact ws
+
+
+-- # Chomp
+
+def Chomp (height length : ℕ) : zSymm_Game_World (Finset (ℕ × ℕ)) (ℕ × ℕ) where
+  toSymm_Game_World := preChomp height length
+  hgw := preChomp_isWL height length
+  hgp := preChomp_playable height length
+  hgn := preChomp_coherent_end height length
+
+
+
+
+-- # Bait
+
+
+lemma Chomp_state_empty_not_empty (height length : ℕ) : ¬Chomp_state (Chomp_init height length) [] = ∅ :=
+  by rw [Chomp_state_empty] ; rw [← ne_eq ,← Finset.nonempty_iff_ne_empty] ; use (length, height) ; apply Chomp_init_has_len_hei
+
+lemma Bait_leg_fst (height length : ℕ) : (Chomp height length).law [] (length, height) :=
   by
   dsimp [Chomp, preChomp]
-  rw [if_pos ⟨Chomp_init_has_zero _ _ , (by trivial)⟩ ]
-  rw [Chomp_state_empty]
-  rw [if_pos (by intro con ; have := Chomp_init_has_len_hei height length ; rw [con, Finset.mem_singleton, Prod.eq_iff_fst_eq_snd_eq] at this ; cases' h with h h ; exact h this.2 ; exact h this.1 )]
+  rw [if_pos (by apply Chomp_state_empty_not_empty)]
   constructor
-  · exact Chomp_init_has_len_hei height length
-  · intro q qdef ; contradiction
-  · apply List.Pairwise.nil
-  · intro q qdef ; contradiction
-  · intro con ; rw [Prod.eq_iff_fst_eq_snd_eq] at con ; cases' h with h h ; exact h con.2 ; exact h con.1
+  · apply Chomp_init_has_len_hei
+  · intro _ no
+    contradiction
 
-
-lemma Chomp_state_zero_top (height length : ℕ) (hist : List (ℕ × ℕ))
-  (hh : hist ≠ []) (hm : ∀ q ∈ hist, q ∈ Chomp_init height length):
-  Chomp_state (Chomp_init height length) hist = {(0, 0)} ↔ Chomp_state (Chomp_init height length) (hist ++ [(length, height)]) = {(0, 0)}  :=
+lemma Bait_leg_imp {height length : ℕ} (h : height ≠ 0 ∨ length ≠ 0) :
+  ∀ hist, ∀ act, (Chomp height length).hist_legal (hist) →
+    (Chomp height length).law (hist ++ [(length, height)]) act → (Chomp height length).law (hist) act :=
   by
-  cases' hist with x l
-  · contradiction
-  · have main : Chomp_state (Chomp_init height length) (x :: l) =  Chomp_state (Chomp_init height length) ((x :: l) ++ [(length, height)]) :=
-      by
-      dsimp [Chomp_state]
-      apply Finset.filter_congr
-      intro y _
-      constructor
-      · intro Q q qdef
-        rw [← List.cons_append, List.mem_append] at qdef
-        cases' qdef with qdef qdef
-        · exact Q _ qdef
-        · rw [List.mem_singleton] at qdef
-          rw [qdef]
-          specialize Q x (by exact List.mem_cons_self x l)
-          specialize hm x (by exact List.mem_cons_self x l)
-          simp_rw [Chomp_init, Finset.mem_product, Finset.mem_range, Nat.lt_succ] at hm
-          dsimp [nondomi, domi] at *
-          contrapose! Q
-          exact ⟨le_trans hm.1 Q.1,  le_trans hm.2 Q.2⟩
-      · intro Q q qdef
-        rw [← List.cons_append] at Q
-        apply Q
-        exact List.mem_append_left [(length, height)] qdef
-    rw [main]
+  intro hist act _ leg
+  dsimp [Chomp, preChomp]
+  dsimp [Chomp, preChomp] at leg
+  split_ifs with S
+  rw [if_pos] at leg
+  · constructor
+    · exact leg.act_mem
+    · intro q qh
+      exact leg.nd q (by apply List.mem_append_left ; exact qh)
+  · contrapose! S
+    apply Chomp_state_hist_zero
+    replace S := Chomp_state_state_empty _ (by apply Chomp_init_has_zero) _ S
+    rw [List.mem_append] at S
+    cases' S with S S
+    · exact S
+    · exfalso
+      apply helper _ _ h
+      exact S
 
 
-
-lemma Chomp_state_zero_append_non_zero (ini : Finset (ℕ × ℕ)) (hist : List (ℕ × ℕ)) (act : ℕ × ℕ)
-  (hs : Chomp_state ini hist = {(0,0)}) (ha : act ≠ (0,0)) : Chomp_state ini (hist ++ [act]) = {(0,0)} :=
-  by
-  dsimp [Chomp_state] at *
-  simp_rw [Finset.eq_singleton_iff_unique_mem, Finset.mem_filter] at *
-  refine' ⟨⟨hs.1.1, _ ⟩, _ ⟩
-  · intro q qdef
-    rw [List.mem_append] at qdef
-    cases' qdef with qdef qdef
-    · exact hs.1.2 q qdef
-    · rw [List.mem_singleton] at qdef
-      rw [qdef]
-      intro con
-      dsimp [domi] at con
-      simp_rw [Nat.le_zero] at con
-      apply ha
-      rw [Prod.eq_iff_fst_eq_snd_eq]
-      exact con
-  · intro x ⟨xi, xd⟩
-    apply hs.2
-    refine' ⟨ xi, _ ⟩
-    intro q qdef
-    apply xd
-    exact List.mem_append.mpr (Or.inl qdef)
-
-
-lemma Chomp_init_has_top (height length : ℕ) : (length, height) ∈ Chomp_init height length :=
-  by
-  simp_rw [Chomp_init, Finset.mem_product, Finset.mem_range, Nat.lt_succ]
-  refine' ⟨ le_refl length , le_refl height ⟩
-
-
-
-
-lemma fst_stolen_act_mem_init (height length : ℕ)
-  (ws s_strat : Strategy (Finset (ℕ × ℕ)) (ℕ × ℕ)) (t : Nat) (tf : Turn_fst (Nat.succ t + 1))
-  (leg : Chomp_law (Chomp_init height length)
-      (History_on_turn (Chomp_init height length) (stolen_strat (length, height) ws) s_strat t)
-      (s_strat (Chomp_init height length)
-        (History_on_turn (Chomp_init height length) (stolen_strat (length, height) ws) s_strat t))) :
-  ws (Chomp_init height length) [(length, height)] ∈ Chomp_init height length :=
-  by
-  cases' t with t
-  · contradiction
-  · have := History_on_turn_stolen_getLast (Chomp_init height length) (length, height) ws s_strat t
-    rw [← this]
-    apply leg.hist_mem
-    apply List.getLast_mem
-
-
-lemma pre_stolen_strat_legal_fst_helper_1 (height length : ℕ) (a b : Nat × Nat)
+lemma nondomi_len_hei {height length : ℕ} (a b : Nat × Nat)
   (adef : a ∈ Chomp_init height length) (bdef : b ∈ Chomp_init height length)
   (main : nondomi b a) : nondomi (length, height) a :=
   by
@@ -1683,167 +593,164 @@ lemma pre_stolen_strat_legal_fst_helper_1 (height length : ℕ) (a b : Nat × Na
   · exact le_antisymm adef.1 main.1
   · exact le_antisymm adef.2 main.2
 
-lemma pre_stolen_strat_legal_fst_helper_2 (height length : ℕ) (act : Nat × Nat) (hist : List (Nat × Nat))
-  (hh : hist ≠ [])
-  (leg : Chomp_law (Chomp_init height length) hist act)
-  (x : Nat × Nat) (xdef : x ∈ hist) : nondomi (length, height) x :=
+lemma Bait_leg_imp' {height length : ℕ} (h : height ≠ 0 ∨ length ≠ 0) :
+  ∀ hist, ∀ act, (Chomp height length).hist_legal (hist) →
+    (Z : ¬ hist = []) → hist.getLast Z = (length, height) → Turn_fst (hist.length + 1) → (Chomp height length).law hist.dropLast act → (Chomp height length).law hist act :=
   by
-  have := leg.hist_nd
-  rw [← List.dropLast_append_getLast hh, List.pairwise_append] at this
-  rw [← List.dropLast_append_getLast hh, List.mem_append] at xdef
-  cases' xdef with xdef xdef
-  · replace this := this.2.2 _ xdef (List.getLast hist hh) (by exact List.mem_singleton.mpr rfl)
-    apply pre_stolen_strat_legal_fst_helper_1 _ _ _ _ _ _ this
-    · apply leg.hist_mem
-      exact List.mem_of_mem_dropLast xdef
-    · apply leg.hist_mem
-      exact List.getLast_mem hh
-  · rw [List.mem_singleton] at xdef
-    rw [xdef]
+  intro hist act hist_leg Z L T leg
+  dsimp [Chomp, preChomp]
+  dsimp [Chomp, preChomp] at leg
+  split_ifs with S
+  rw [← List.dropLast_append_getLast Z, L]
+  rw [← List.dropLast_append_getLast Z, L] at S
+  rw [if_pos] at leg
+  · constructor
+    · exact leg.act_mem
+    · intro q qh
+      rw [List.mem_append] at qh
+      cases' qh with qh qh
+      · exact leg.nd _ qh
+      · match hist with
+        | [] => contradiction
+        | [_] => dsimp at T ; contradiction
+        | x :: y :: l =>
+            rw [List.dropLast_cons_of_ne_nil (List.noConfusion)] at leg
+            cases' hist_leg
+            rename_i _ now
+            dsimp at now
+            rw [ite_self] at now
+            dsimp [Chomp, preChomp] at now
+            rw [if_pos] at now
+            · replace now := now.act_mem
+              have amem := leg.act_mem
+              replace leg := leg.nd x (by apply List.mem_cons_self)
+              rw [List.mem_singleton] at qh
+              rw [qh]
+              apply nondomi_len_hei _ x amem now leg
+            · contrapose! S
+              apply Chomp_state_hist_zero
+              replace S := Chomp_state_state_empty _ (by apply Chomp_init_has_zero) _ S
+              rw [List.dropLast_cons_of_ne_nil (List.noConfusion)]
+              apply List.mem_append_left
+              apply List.mem_cons_of_mem
+              have : l ≠ [] := by
+                intro con
+                simp_rw [con] at L S
+                dsimp [List.getLast] at L
+                rw [L] at S
+                apply helper  _ _ h S
+              rw [List.dropLast_cons_of_ne_nil this]
+              rw [← List.dropLast_append_getLast this, ← List.cons_append, List.mem_append] at S
+              cases' S with S S
+              · exact S
+              · exfalso
+                rw [List.getLast_cons (List.noConfusion)] at L
+                rw [List.getLast_cons this] at L
+                rw [L] at S
+                apply helper  _ _ h S
+  · contrapose! S
+    apply Chomp_state_hist_zero
+    replace S := Chomp_state_state_empty _ (by apply Chomp_init_has_zero) _ S
+    exact List.mem_append_left [(length, height)] S
 
 
+lemma Chomp_Bait {height length : ℕ} (h : height ≠ 0 ∨ length ≠ 0) : Bait (Chomp height length) (length, height) :=
+  {leg_fst := Bait_leg_fst height length, leg_imp := Bait_leg_imp h, leg_imp' := Bait_leg_imp' h}
 
 
-
-
-
-
-
---#exit
-
-lemma pre_stolen_strat_legal_fst (height length : ℕ) (h : height ≠ 0 ∨ length ≠ 0)
-  (ws s_strat : Strategy (Finset (ℕ × ℕ)) (ℕ × ℕ))
-  (f_leg : Strategy_legal_snd (Chomp height length).init_game_state (Chomp height length).law (stolen_strat (length, height) ws) s_strat)
-  : Strategy_legal_fst (Chomp height length).init_game_state (Chomp height length).law (pre_stolen_strat (length, height)  s_strat) ws :=
+lemma Chomp_not_init_win {height length : ℕ} : ¬ (Chomp height length).snd_win_states [] :=
   by
-  intro t tf
-  cases' t with t
-  · dsimp!
-    unfold pre_stolen_strat
-    rw [if_pos (by rfl)]
-    apply Chomp_len_heigh_legal _ _ h
-  · rw [← History_on_turn_stolen_pre_stolen]
-    simp only [ne_eq, pre_stolen_strat, List.append_eq_nil, and_false, List.dropLast_concat, ite_false]
-    have f_leg' := f_leg t (by rw [Turn_snd_fst_step] ; exact tf)
-    dsimp [Chomp, preChomp]
-    dsimp [Chomp, preChomp] at f_leg'
-    have : History_on_turn (Chomp_init height length) (stolen_strat (length, height) ws) s_strat t ≠ [] :=
-        by
-        cases' t with t
-        · contradiction
-        · apply History_on_turn_nonempty_of_succ
-    by_cases qwlog : (0, 0) ∈ History_on_turn (Chomp_init height length) (stolen_strat (length, height) ws) s_strat t
-    · rw [if_neg (by rw [not_and_or,not_not] ; right ; apply List.mem_append_left ; exact qwlog )]
-      exact trivial
-    · rw [if_pos ⟨Chomp_init_has_zero _ _, qwlog⟩] at f_leg'
-      rw [if_pos ⟨Chomp_init_has_zero _ _, (by apply List.not_mem_append qwlog (helper _ _ h))⟩]
-      by_cases q : ¬Chomp_state (Chomp_init height length) (History_on_turn (Chomp_init height length) (stolen_strat (length, height) ws) s_strat t) = {(0, 0)}
-      · rw [if_pos q] at f_leg'
-        replace this := Chomp_state_zero_top height length _ this f_leg'.hist_mem
-        rw [← not_iff_not] at this
-        rw [this] at q
-        rw [if_pos q]
-        constructor
-        · exact f_leg'.act_mem
-        · intro q qdef
-          rw [List.mem_append] at qdef
-          cases' qdef with qdef qdef
-          · exact f_leg'.hist_mem q qdef
-          · rw [List.mem_singleton] at qdef
-            rw [qdef]
-            apply Chomp_init_has_top
-        · rw [List.pairwise_append]
-          refine' ⟨(by apply f_leg'.hist_nd), (by apply List.pairwise_singleton), _ ⟩
-          intro a adef b bdef
-          rw [List.mem_singleton] at bdef
-          rw [bdef]
-          sorry
-        · intro a adef
-          rw [List.mem_append] at adef
-          cases' adef with adef adef
-          · exact f_leg'.nd _ adef
-          · rw [List.mem_singleton] at adef
-            rw [adef]
-            have : nondomi (ws (Chomp_init height length) [(length, height)]) (s_strat (Chomp_init height length) (History_on_turn (Chomp_init height length) (stolen_strat (length, height) ws) s_strat t)) :=
-              by
-              apply f_leg'.nd
-              cases' t with t
-              · contradiction
-              · rw [← History_on_turn_stolen_getLast (Chomp_init height length) (length, height) ws s_strat t]
-                apply List.getLast_mem
-            apply pre_stolen_strat_legal_fst_helper_1 _ _ _ _ (f_leg'.act_mem) (fst_stolen_act_mem_init _ _ _ _ _ tf f_leg') this
-        · exact f_leg'.nz_act
-      · rw [if_neg q] at f_leg'
-        rw [not_not] at q
-        replace q := Chomp_state_zero_append_non_zero _ _ (length, height) q (by intro con ; rw [Prod.eq_iff_fst_eq_snd_eq] at con ; cases' h with h h ; apply h ; exact con.2 ; apply h ; exact con.1)
-        rw [if_neg (by rw [not_not]; apply q)]
-        exact f_leg'
+  dsimp [Chomp, preChomp, Chomp_win_snd]
+  push_neg
+  intro h a _ con
+  replace con := con.ref
+  rw [List.suffix_nil] at con
+  contradiction
 
 
 
--- trouble on whether act isn't (len, height) → hist non empty, and act legal should imply it...
 
 
-lemma Strong_strategy_stealing (height length : ℕ) (h : height ≠ 0 ∨ length ≠ 0) : (Chomp height length).is_fst_win :=
+lemma List.ne_empty_of_mem {l : List α} {x : α} (h : x ∈ l) : l ≠ [] := by
+  cases' l with _ _
+  · contradiction
+  · apply List.noConfusion
+
+
+lemma List.singleton_suffix  {l : List α} {x : α} (h : [x] <:+ l) : x = l.getLast (List.ne_empty_of_mem (List.mem_of_suffix h (List.mem_cons_self x []))) := by
+  obtain ⟨t,td⟩ := h ; simp_rw [← td, List.getLast_append]
+
+
+lemma Chomp_winning_equiv {height length : ℕ} (H : height ≠ 0 ∨ length ≠ 0) :
+  ∀ hist, (Chomp height length).hist_legal hist → (Chomp height length).snd_win_states (hist ++ [(length, height)]) → (Chomp height length).fst_win_states hist :=
   by
-  cases' (zSymm_Game_World.Zermelo (Chomp height length) (Chomp_WLT _ _ h)) with F S
-  · exact F
-  · obtain ⟨ws, ws_prop⟩ := S
-    use (stolen_strat (length, height) ws)
-    intro s_strat s_leg
-
--- TODO : replace wining strat def so that request ∀ t, leg f at t → leg ws at (t+1) ...
-
-
--- initial stealing stuff
-#exit
-lemma Chomp_Stealing_condition (height length : ℕ) (h : height ≠ 0 ∨ length ≠ 0) : Strong_stealing_condition (Chomp height length) :=
-  by
-  use (length, height)
+  intro h _
+  intro q
+  dsimp [Chomp, preChomp, Chomp_win_fst, Chomp_win_snd] at *
+  obtain ⟨hist,act,T,W⟩ := q
+  use (hist.dropLast)
+  use act
+  have fact : hist ≠ [] :=
+    by
+    intro con
+    rw [con] at W
+    have oh := W.ref
+    have no := W.F
+    replace oh := List.singleton_suffix oh
+    rw [List.getLast_append] at oh
+    rw [oh] at no
+    replace no := Chomp_state_state_empty _ (Chomp_init_has_zero height length) _ no
+    apply helper _ _ H no
+  have : hist = hist.dropLast ++ [(length,height)] :=
+    by
+    nth_rewrite 1 [← List.dropLast_append_getLast fact]
+    congr
+    obtain ⟨t,tdef⟩ := W.ref
+    have : List.getLast (t ++ act :: hist) (by apply List.append_ne_nil_of_ne_nil_right ; apply List.noConfusion) = List.getLast (h ++ [(length, height)]) (by apply List.append_ne_nil_of_ne_nil_right ; apply List.noConfusion) := by simp_rw [tdef]
+    simp_rw [List.getLast_append] at this
+    simp_rw [List.getLast_append' t (act :: hist) List.noConfusion] at this
+    simp_rw [List.getLast_cons fact] at this
+    exact this
   constructor
-  · dsimp [Chomp, preChomp]
-    rw [if_pos ⟨Chomp_init_has_zero _ _ , (by trivial)⟩ ]
-    rw [Chomp_state_empty]
-    rw [if_pos (by intro con ; have := Chomp_init_has_len_hei height length ; rw [con, Finset.mem_singleton, Prod.eq_iff_fst_eq_snd_eq] at this ; cases' h with h h ; exact h this.2 ; exact h this.1 )]
-    constructor
-    · exact Chomp_init_has_len_hei height length
-    · intro q qdef ; contradiction
-    · apply List.Pairwise.nil
-    · intro q qdef ; contradiction
-    · intro con ; rw [Prod.eq_iff_fst_eq_snd_eq] at con ; cases' h with h h ; exact h con.2 ; exact h con.1
-  · intro act hist leg hne htop
-    constructor
-    · apply preChomp_law_prop_transition _ _ h _ _ leg
-    · apply preChomp_law_prop_law _ _ h _ _ hne htop leg
+  · rw [List.length_dropLast, Nat.sub_add_cancel (by rw [Nat.succ_le, List.length_pos] ; apply fact), Turn_snd_fst_step] ; exact T
+  · constructor
+    · intro con
+      apply W.N
+      rw [← Finset.subset_empty] at *
+      rw [← List.dropLast_append_getLast fact]
+      apply Finset.Subset.trans _ con
+      apply Chomp_state_sub
+    · apply Chomp_state_hist_zero
+      have that := Chomp_state_state_empty _ (Chomp_init_has_zero height length) _ W.F
+      rw [this, ← List.cons_append, List.mem_append] at that
+      cases' that with q q
+      · exact q
+      · exfalso
+        apply helper _ _ H q
+    · replace W := W.ref
+      rw [this, ← List.cons_append] at W
+      obtain ⟨t,td⟩ := W
+      rw [← List.append_assoc] at td
+      replace td := List.append_inj_left' td rfl
+      use t
+
+/--
+Chomp satisfies the stealing conditions.
+
+Suppose the second player has a winning strategy. The frist player may steal it as follows.
+The frist player considers playing the top-most outer-most tile of the board, and considers the response of the second player.
+The frist player can play that response from the start, pretending to be the second player, acting as if the actual player
+was the first player and had played the top-most outer-most tile as a first move.
+-/
+lemma Chomp_stealing_condition {height length : ℕ} (H : height ≠ 0 ∨ length ≠ 0) : Stealing_condition (Chomp height length) where
+  trap := (length, height)
+  hb := Chomp_Bait H
+  fst_not_win := Chomp_not_init_win
+  wb := Chomp_winning_equiv H
 
 
---#exit
-
-lemma pre_stolen_strat_legal_fst (height length : ℕ) (h : height ≠ 0 ∨ length ≠ 0) --(hgu : g.strat_unique_actions)
-  (ws s_strat : Strategy (Finset (ℕ × ℕ)) (ℕ × ℕ))
-  (f_leg : Strategy_legal_snd (Chomp height length).init_game_state (Chomp height length).law (stolen_strat (Chomp height length) (Chomp_Stealing_condition _ _ h) ws) s_strat)
-  : Strategy_legal_fst (Chomp height length).init_game_state (Chomp height length).law (pre_stolen_strat (Chomp height length) (Chomp_Stealing_condition _ _ h) s_strat) ws :=
+theorem Chomp_is_fst_win {height length : ℕ} (H : height ≠ 0 ∨ length ≠ 0) :
+  (Chomp height length).is_fst_win  :=
   by
-  intro t tf
-  cases' t with t
-  · dsimp!
-    unfold pre_stolen_strat
-    rw [if_pos (by rfl)]
-    apply (Classical.choose_spec (Chomp_Stealing_condition _ _ h)).1
-  · rw [← History_on_turn_stolen_pre_stolen]
-    simp only [ne_eq, pre_stolen_strat, List.append_eq_nil, and_false, List.dropLast_concat, ite_false]
-    have f_leg' := f_leg t (by rw [Turn_snd_fst_step] ; exact tf)
-    dsimp [Chomp, preChomp]
-    dsimp [Chomp, preChomp] at f_leg'
-
-  -- induction' t with t ih
-  -- · dsimp!
-  --   unfold pre_stolen_strat
-  --   rw [if_pos (by rfl)]
-  --   apply (Classical.choose_spec (Chomp_Stealing_condition _ _ h)).1
-  -- · rw [← History_on_turn_stolen_pre_stolen]
-  --   simp only [ne_eq, pre_stolen_strat, List.append_eq_nil, and_false, List.dropLast_concat, ite_false]
-  --   have f_leg' := f_leg t (by rw [Turn_snd_fst_step] ; exact tf)
-  --   cases' t with t
-  --   · contradiction
-  --   · sorry
+  apply Strategy_stealing
+  apply Chomp_stealing_condition H
